feat (sorting) tidy up Introsort

thys/examples/sorting/Sorting_Final_insertion_Sort.thy
@@ -1,23 +1,38 @@
+section \<open>Final Insertion Sort\<close>
 theory Sorting_Final_insertion_Sort
 imports Sorting_Quicksort_Scheme Sorting_Unguarded_Insertion_Sort
 begin
 
+
+
+(* TODO: move*)
+lemma nrest_le_formatI:
+  fixes a :: "(_,(_,enat)acost) nrest"
+  shows  "a \<le> \<Down>Id (timerefine TId b) \<Longrightarrow> a \<le> b"
+  by (auto simp add: timerefine_id)
+
+
+
 context weak_ordering begin
+
+subsection \<open>final_insertion_sort\<close>
 
   definition "final_insertion_sort xs \<equiv> doN {
     ASSERT (1 < length xs);
     lxs \<leftarrow> SPECT [length xs \<mapsto> cost ''sub'' 1];
     if\<^sub>N SPECc2 ''icmp_sle'' (\<le>) lxs is_threshold then doN {
       SPECT [() \<mapsto> cost ''add'' 1];
-      gen_insertion_sort_guarded 1 lxs xs
+      insertion_sort_guarded 1 lxs xs
     }
     else doN {
       SPECT [() \<mapsto> cost ''add'' 2];
-      xs \<leftarrow> gen_insertion_sort_guarded 1 is_threshold xs;
-      gen_insertion_sort_unguarded is_threshold is_threshold lxs xs
+      xs \<leftarrow> insertion_sort_guarded 1 is_threshold xs;
+      insertion_sort_unguarded is_threshold is_threshold lxs xs
     }
   }"  
 
+
+subsubsection \<open>reasoning about stopper elements\<close>
 
   lemma has_stopperI:
     assumes "i<length xs" "j'<i" "i-j'\<le>N" "\<forall>j\<le>j'. \<not>xs!i\<^bold><xs!j"
@@ -118,21 +133,13 @@ context weak_ordering begin
     assumes "mset (slice 0 N xs') = mset (slice 0 N xs)"
     assumes "j < N" "N < length xs" "length xs' = length xs"
     obtains jj where "jj<N" "xs'!j = xs!jj"
-    using assms by (auto simp: list_eq_iff_nth_eq set_slice_conv dest!: mset_eq_setD; auto) 
-  
-    
-    
-  find_theorems sorted_wrt mset
-  
-  find_consts "_ multiset \<Rightarrow> nat"
-  
+    using assms by (auto simp: list_eq_iff_nth_eq set_slice_conv dest!: mset_eq_setD; auto)       
   
   lemma filter_mset_eq_empty_conv: "filter_mset P m = {#} \<longleftrightarrow> (\<forall>x\<in>#m. \<not>P x)"
     by (auto simp: filter_mset_eq_conv)
   
   lemma filter_mset_eq_same_conv: "filter_mset P m = m \<longleftrightarrow> (\<forall>x\<in>#m. P x)"
-    by (auto simp: filter_mset_eq_conv)
-    
+    by (auto simp: filter_mset_eq_conv)    
     
   lemma sorted_pos_aux:
     assumes "size (filter_mset (\<lambda>x. x \<^bold>\<le> a) (mset xs)) \<ge> n" "sorted_wrt (\<^bold>\<le>) xs"
@@ -165,10 +172,8 @@ context weak_ordering begin
       also have "length xs\<^sub>1 < n" unfolding xs\<^sub>1_def using \<open>i<n\<close> NL by auto
       finally show False using assms(1) by simp
     qed
-  qed  
-       
-  
-  
+  qed
+
   lemma filter_mset_eq_sameI: 
     "(\<forall>x\<in>#m. P x) \<Longrightarrow> filter_mset P m = m" by (simp add: filter_mset_eq_same_conv)
   
@@ -212,9 +217,7 @@ context weak_ordering begin
       using LE by (simp add: Misc.slice_def)
     thus ?thesis using LE by (auto simp: unfold_le_to_lt)
   qed    
-      
-      
-    
+
   lemma transfer_stopper_over_initial_sorting:
     assumes "has_stopper N xs i"
     assumes B: "length xs' = length xs" "0<N" "N \<le> i" "i < length xs"
@@ -255,43 +258,37 @@ context weak_ordering begin
     using assms transfer_stopper_over_initial_sorting part_sorted_guardedI by blast
 
 
-  term slice_sort_specT
-lemma puulla: "slice_sort_specT (enat (h-i\<^sub>0+1) *m insort_guarded_step_cost) (\<^bold><) xs 0 h
-  = \<Down>Id (timerefine (TId(''slice_sort'' := enat (h-i\<^sub>0+1) *m insort_guarded_step_cost)) (
-          slice_sort_spec (\<^bold><) xs 0 h))"
-  unfolding slice_sort_spec_def slice_sort_specT_def
-  apply(cases "h \<le> length xs"; auto)
-  apply(simp add: SPEC_timerefine_conv) 
-  apply(rule SPEC_cong, simp)
-  by(simp add: timerefineA_cost) 
+  lemma pull_refinement_into_slice_sort_specT:
+    "slice_sort_specT (enat (h-i\<^sub>0+1) *m insort_guarded_step_cost) (\<^bold><) xs 0 h
+      = \<Down>Id (timerefine (TId(''slice_sort'' := enat (h-i\<^sub>0+1) *m insort_guarded_step_cost)) (
+            slice_sort_spec (\<^bold><) xs 0 h))"
+    unfolding slice_sort_spec_def slice_sort_specT_def
+    apply(cases "h \<le> length xs"; auto)
+    apply(simp add: SPEC_timerefine_conv) 
+    apply(rule SPEC_cong, simp)
+    by(simp add: timerefineA_cost) 
   
 
   abbreviation "guarded_insort_cost lxs \<equiv> enat (lxs+1) *m insort_guarded_step_cost"
 
-  lemma gen_insertion_sort_guarded_correct_fl: 
+  lemma insertion_sort_guarded_correct_fl: 
     "\<lbrakk>sorted_wrt_lt (\<^bold><) (take i\<^sub>0 xs); h\<le>length xs ; i\<^sub>0<h; h\<le>length xs \<rbrakk> 
-      \<Longrightarrow> gen_insertion_sort_guarded i\<^sub>0 h xs 
+      \<Longrightarrow> insertion_sort_guarded i\<^sub>0 h xs 
         \<le> slice_sort_specT (guarded_insort_cost (h-i\<^sub>0)) (\<^bold><) xs 0 h"
-    apply(subst puulla)
-    apply(rule gen_insertion_sort_guarded_correct)                    
+    apply(subst pull_refinement_into_slice_sort_specT)
+    apply(rule insertion_sort_guarded_correct)                    
        apply auto
     done
 
 
-(* TODO: move*)
-lemma nrest_le_formatI:
-  fixes a :: "(_,(_,enat)acost) nrest"
-  shows  "a \<le> \<Down>Id (timerefine TId b) \<Longrightarrow> a \<le> b"
-  by (auto simp add: timerefine_id)
 
 
-
-  lemma gen_insertion_sort_guarded_correct_threshold: 
+  lemma insertion_sort_guarded_correct_threshold: 
     "\<lbrakk>sorted_wrt_lt (\<^bold><) (take i\<^sub>0 xs); h\<le>length xs ; i\<^sub>0<h; h\<le>length xs; (h-i\<^sub>0)\<le>is_threshold \<rbrakk> 
-      \<Longrightarrow> gen_insertion_sort_guarded i\<^sub>0 h xs 
+      \<Longrightarrow> insertion_sort_guarded i\<^sub>0 h xs 
         \<le> slice_sort_specT (guarded_insort_cost is_threshold) (\<^bold><) xs 0 h"
     apply(rule order_trans)
-     apply(rule gen_insertion_sort_guarded_correct_fl)
+     apply(rule insertion_sort_guarded_correct_fl)
         apply auto [4]
     unfolding slice_sort_specT_def
     apply(rule nrest_le_formatI)
@@ -300,39 +297,41 @@ lemma nrest_le_formatI:
     apply(rule costmult_right_mono)
     by auto
 
-lemma brr: "\<lbrakk>sorted_wrt_lt (\<^bold><) (take i\<^sub>0 xs\<^sub>0); h \<le> length xs\<^sub>0; i\<^sub>0 < h; h \<le> length xs\<^sub>0; h - i\<^sub>0 \<le> is_threshold;
+  lemma final_insertion_sort_correct_aux:
+    "\<lbrakk>sorted_wrt_lt (\<^bold><) (take i\<^sub>0 xs\<^sub>0); h \<le> length xs\<^sub>0; i\<^sub>0 < h; h \<le> length xs\<^sub>0; h - i\<^sub>0 \<le> is_threshold;
           0 \<le> h \<and> h \<le> length xs\<^sub>0\<rbrakk>
-  \<Longrightarrow> gen_insertion_sort_guarded i\<^sub>0 h xs\<^sub>0 \<le> 
+    \<Longrightarrow> insertion_sort_guarded i\<^sub>0 h xs\<^sub>0 \<le> 
         SPECT
          (emb (\<lambda>xs. length xs = length xs\<^sub>0 \<and> take 0 xs = take 0 xs\<^sub>0 \<and> drop h xs = drop h xs\<^sub>0 \<and> sort_spec (\<^bold><) (slice 0 h xs\<^sub>0) (slice 0 h xs))
            (guarded_insort_cost is_threshold))
       "
-  using gen_insertion_sort_guarded_correct_threshold[of i\<^sub>0 xs\<^sub>0 h]
+  using insertion_sort_guarded_correct_threshold[of i\<^sub>0 xs\<^sub>0 h]
   unfolding slice_sort_specT_def SPEC_REST_emb'_conv
   by(cases "0 \<le> h \<and> h \<le> length xs\<^sub>0", auto)
 
 
   abbreviation "unguarded_insort_cost lxs \<equiv> enat (lxs+1) *m insort_step_cost"
 
-  thm gen_insertion_sort_unguarded_correct
+  thm insertion_sort_unguarded_correct
 
-lemma puulla_guarded: "slice_sort_specT (enat (h-i\<^sub>0+1) *m insort_step_cost) (\<^bold><) xs 0 h
-  = \<Down>Id (timerefine (TId(''slice_sort'' := enat (h-i\<^sub>0+1) *m insort_step_cost)) (
-          slice_sort_spec (\<^bold><) xs 0 h))"
-  unfolding slice_sort_spec_def slice_sort_specT_def
-  apply(cases "h \<le> length xs"; auto)
-  apply(simp add: SPEC_timerefine_conv) 
-  apply(rule SPEC_cong, simp)
-  by(simp add: timerefineA_cost) 
+  lemma pull_refinement_into_slice_sort_specT_guarded:
+    "slice_sort_specT (enat (h-i\<^sub>0+1) *m insort_step_cost) (\<^bold><) xs 0 h
+    = \<Down>Id (timerefine (TId(''slice_sort'' := enat (h-i\<^sub>0+1) *m insort_step_cost)) (
+            slice_sort_spec (\<^bold><) xs 0 h))"
+    unfolding slice_sort_spec_def slice_sort_specT_def
+    apply(cases "h \<le> length xs"; auto)
+    apply(simp add: SPEC_timerefine_conv) 
+    apply(rule SPEC_cong, simp)
+    by(simp add: timerefineA_cost) 
 
-  lemma gen_insertion_sort_unguarded_correct_prepared: 
+  lemma insertion_sort_unguarded_correct_prepared: 
     "\<lbrakk>sorted_wrt_lt (\<^bold><) (take i\<^sub>0 xs\<^sub>0); (\<forall>i\<in>{i\<^sub>0..<h}. has_stopper N xs\<^sub>0 i) \<and> h\<le>length xs\<^sub>0 ; i\<^sub>0<h; h\<le>length xs\<^sub>0 \<rbrakk> 
-      \<Longrightarrow> gen_insertion_sort_unguarded N i\<^sub>0 h xs\<^sub>0 
+      \<Longrightarrow> insertion_sort_unguarded N i\<^sub>0 h xs\<^sub>0 
         \<le> SPECT
          (emb (\<lambda>xs. length xs = length xs\<^sub>0 \<and> take 0 xs = take 0 xs\<^sub>0 \<and> drop h xs = drop h xs\<^sub>0 \<and> sort_spec (\<^bold><) (slice 0 h xs\<^sub>0) (slice 0 h xs))
  (unguarded_insort_cost (h)))"
     apply(rule order.trans)
-     apply(rule gen_insertion_sort_unguarded_correct)
+     apply(rule insertion_sort_unguarded_correct)
         apply auto [4]
     unfolding slice_sort_spec_def slice_sort_specT_def
     apply auto
@@ -344,16 +343,20 @@ lemma puulla_guarded: "slice_sort_specT (enat (h-i\<^sub>0+1) *m insort_step_cos
     done
 
 
+  
+  abbreviation "fi_cost lxs == guarded_insort_cost (is_threshold)
+         + cost ''add'' 1 + cost ''add'' 1
+        + cost ''if'' 1 +  cost ''sub'' 1 + cost ''icmp_sle'' 1
+        + unguarded_insort_cost lxs
+      "
 
-abbreviation "fi_cost lxs == guarded_insort_cost (is_threshold)
-       + cost ''add'' 1 + cost ''add'' 1
-      + cost ''if'' 1 +  cost ''sub'' 1 + cost ''icmp_sle'' 1
-      + unguarded_insort_cost lxs
-    "
+  subsubsection \<open>Correctness Theorem\<close>
 
   lemma final_insertion_sort_correct: 
     "\<lbrakk>part_sorted_wrt (le_by_lt (\<^bold><)) is_threshold xs; 1 < length xs; lxs=length xs\<rbrakk> 
-      \<Longrightarrow> final_insertion_sort xs \<le> \<Down>Id (timerefine (TId(''sort_spec'':=fi_cost lxs)) (SPEC (sort_spec (\<^bold><) xs) (\<lambda>_. cost ''sort_spec'' 1)))"
+      \<Longrightarrow> final_insertion_sort xs
+       \<le> \<Down>Id (timerefine (TId(''sort_spec'':=fi_cost lxs))
+               (SPEC (sort_spec (\<^bold><) xs) (\<lambda>_. cost ''sort_spec'' 1)))"
     unfolding final_insertion_sort_def SPEC_timerefine_conv
     apply simp
     unfolding SPEC_def
@@ -362,8 +365,7 @@ abbreviation "fi_cost lxs == guarded_insort_cost (is_threshold)
     apply (refine_vcg \<open>-\<close>)
 
     subgoal (* if branch *)
-      apply(rule brr[THEN gwp_specifies_rev_I, THEN gwp_conseq_0 ])
-      thm  brr[THEN gwp_specifies_rev_I, THEN gwp_conseq_0 ]
+      apply(rule final_insertion_sort_correct_aux[THEN gwp_specifies_rev_I, THEN gwp_conseq_0 ])
 
     apply simp_all
       subgoal apply (rule sorted_wrt01) by auto  
@@ -374,10 +376,10 @@ abbreviation "fi_cost lxs == guarded_insort_cost (is_threshold)
       apply sc_solve by (auto simp: one_enat_def)
 
     subgoal (* else branch *)
-      apply(rule brr[THEN gwp_specifies_rev_I, THEN gwp_conseq_0 ])
+      apply(rule final_insertion_sort_correct_aux[THEN gwp_specifies_rev_I, THEN gwp_conseq_0 ])
       apply simp_all
       subgoal apply (rule sorted_wrt01) by auto  
-      apply(rule gen_insertion_sort_unguarded_correct_prepared[THEN gwp_specifies_rev_I, THEN gwp_conseq_0 ])
+      apply(rule insertion_sort_unguarded_correct_prepared[THEN gwp_specifies_rev_I, THEN gwp_conseq_0 ])
       apply(simp_all add: emb_eq_Some_conv)
       subgoal by (simp add: Misc.slice_def sort_spec_def) 
       subgoal for xs' t M (* transfer guard over initial sorting *)
@@ -398,18 +400,20 @@ abbreviation "fi_cost lxs == guarded_insort_cost (is_threshold)
     done    
   done
 
+subsection \<open>final_insertion_sort2\<close>
+
   definition "final_insertion_sort2 xs l h \<equiv> doN {
     ASSERT (l<h);
     lxs \<leftarrow> SPECc2 ''sub'' (-) h l;
     if\<^sub>N SPECc2 ''icmp_sle'' (\<le>) lxs is_threshold then do {
       l' \<leftarrow> SPECc2 ''add'' (+) l 1;
-      gen_insertion_sort_guarded2 l l' h xs
+      insertion_sort_guarded2 l l' h xs
     }
     else doN {
       l' \<leftarrow> SPECc2 ''add'' (+) l 1;
       l'' \<leftarrow> SPECc2 ''add'' (+) l is_threshold;
-      xs \<leftarrow> gen_insertion_sort_guarded2 l l' l'' xs;
-      gen_insertion_sort_unguarded2 is_threshold l'' h xs
+      xs \<leftarrow> insertion_sort_guarded2 l l' l'' xs;
+      insertion_sort_unguarded2 is_threshold l'' h xs
     }
   }"  
 
@@ -426,17 +430,17 @@ lemma sp_TR_fi2[simp]: "struct_preserving (TR_fi2 N)"
   
   (* TODO: make these refinement steps use the correct TimeRefine *)
 
-  thm gen_insertion_sort_guarded2_refine
-  lemma gen_insertion_sort_guarded2_refine_prepared: 
+  thm insertion_sort_guarded2_refine
+  lemma insertion_sort_guarded2_refine_prepared: 
     "\<lbrakk> (xsi,xs) \<in> slicep_rel l h; (ii,i)\<in>idx_shift_rel l; (ji,j)\<in>idx_shift_rel l; j\<le>N \<rbrakk> 
-      \<Longrightarrow> gen_insertion_sort_guarded2 l ii ji xsi \<le>\<Down>(slice_rel xsi l h) (timerefine (TR_fi2 N) (gen_insertion_sort_guarded i j xs))"
-    apply(rule gen_insertion_sort_guarded2_refine)
+      \<Longrightarrow> insertion_sort_guarded2 l ii ji xsi \<le>\<Down>(slice_rel xsi l h) (timerefine (TR_fi2 N) (insertion_sort_guarded i j xs))"
+    apply(rule insertion_sort_guarded2_refine)
     apply auto done
 
-  lemma gen_insertion_sort_unguarded2_refine_prepared: 
+  lemma insertion_sort_unguarded2_refine_prepared: 
     "\<lbrakk> (xsi,xs) \<in> slicep_rel l h; (ii,i)\<in>idx_shift_rel l; (ji,j)\<in>idx_shift_rel l \<rbrakk> 
-      \<Longrightarrow> gen_insertion_sort_unguarded2 N ii ji xsi \<le>\<Down>(slice_rel xsi l h) (timerefine (TR_fi2 N) (gen_insertion_sort_unguarded N i j xs))"
-    apply(rule gen_insertion_sort_unguarded2_refine)
+      \<Longrightarrow> insertion_sort_unguarded2 N ii ji xsi \<le>\<Down>(slice_rel xsi l h) (timerefine (TR_fi2 N) (insertion_sort_unguarded N i j xs))"
+    apply(rule insertion_sort_unguarded2_refine)
     apply auto done
 
 
@@ -447,8 +451,8 @@ lemma sp_TR_fi2[simp]: "struct_preserving (TR_fi2 N)"
     unfolding SPECc2_alt consume_RETURNT[symmetric] 
     apply normalize_blocks
 
-    supply [refine] = gen_insertion_sort_guarded2_refine_prepared
-                        gen_insertion_sort_unguarded2_refine_prepared
+    supply [refine] = insertion_sort_guarded2_refine_prepared
+                        insertion_sort_unguarded2_refine_prepared
 
     apply (refine_rcg bindT_refine_conc_time_my_inres MIf_refine consumea_refine) 
     apply refine_dref_type
@@ -470,23 +474,28 @@ lemma sp_TR_fi2[simp]: "struct_preserving (TR_fi2 N)"
       apply sc_solve by simp
     subgoal 
         apply (subst slice_rel_rebase, assumption)
-      apply(refine_rcg gen_insertion_sort_unguarded2_refine_prepared)
+      apply(refine_rcg insertion_sort_unguarded2_refine_prepared)
       by (auto simp: slice_rel_alt idx_shift_rel_def slicep_rel_def) 
     done
 
+  
+  abbreviation "fi2_cost s \<equiv> enat 17 *m TR_is_insert3 is_threshold ''icmp_slt''
+         + enat 17 *m TR_is_insert3 is_threshold ''add''
+           + enat 17 *m TR_is_insert3 is_threshold ''is_insert_g''
+           + enat 17 *m TR_is_insert3 is_threshold ''call'' +
+          enat 17 *m TR_is_insert3 is_threshold ''if'' +
+          TR_is_insert3 is_threshold ''add'' +
+          TR_is_insert3 is_threshold ''add'' +
+          TR_is_insert3 is_threshold ''if'' +
+          TR_is_insert3 is_threshold ''sub'' +
+          TR_is_insert3 is_threshold ''icmp_sle'' +
+          (enat (Suc (s)) *m TR_is_insert3 is_threshold ''icmp_slt''
+             + enat (Suc (s)) *m TR_is_insert3 is_threshold ''add''
+           + enat (Suc (s)) *m TR_is_insert3 is_threshold ''is_insert'' +
+           enat (Suc (s)) *m TR_is_insert3 is_threshold ''call'' +
+           enat (Suc (s)) *m TR_is_insert3 is_threshold ''if'')"
 
-  thm final_insertion_sort2_refine final_insertion_sort_correct
-
-abbreviation "fi2_cost s \<equiv> enat 17 *m TR_is_insert3 is_threshold ''icmp_slt'' + enat 17 *m TR_is_insert3 is_threshold ''add'' + enat 17 *m TR_is_insert3 is_threshold ''is_insert_g'' + enat 17 *m TR_is_insert3 is_threshold ''call'' +
-        enat 17 *m TR_is_insert3 is_threshold ''if'' +
-        TR_is_insert3 is_threshold ''add'' +
-        TR_is_insert3 is_threshold ''add'' +
-        TR_is_insert3 is_threshold ''if'' +
-        TR_is_insert3 is_threshold ''sub'' +
-        TR_is_insert3 is_threshold ''icmp_sle'' +
-        (enat (Suc (s)) *m TR_is_insert3 is_threshold ''icmp_slt'' + enat (Suc (s)) *m TR_is_insert3 is_threshold ''add'' + enat (Suc (s)) *m TR_is_insert3 is_threshold ''is_insert'' +
-         enat (Suc (s)) *m TR_is_insert3 is_threshold ''call'' +
-         enat (Suc (s)) *m TR_is_insert3 is_threshold ''if'')"
+subsubsection \<open>Correctness Theorem\<close>
 
   lemma final_insertion_sort2_correct: 
     assumes [simplified, simp]: "(xs',xs)\<in>Id" "(l',l)\<in>Id" "(h',h)\<in>Id"   
@@ -513,57 +522,11 @@ abbreviation "fi2_cost s \<equiv> enat 17 *m TR_is_insert3 is_threshold ''icmp_s
       apply(subst assms(4)) apply simp
       done
     done
-
-
-lemma fl: 
-  assumes "TR ''slice_sort'' = (enat (h-l+1)) *m cost ''call'' 1"
-  shows  "(timerefine TR (final_sort_spec xs l h))
-        = (timerefine (TId(''slice_sort'':=(enat (h-l+1)) *m cost ''call'' 1)) (final_sort_spec xs l h))"
-  unfolding final_sort_spec_def slice_sort_spec_def
-  apply(cases "1 < h - l \<and> part_sorted_wrt (le_by_lt (\<^bold><)) is_threshold (slice l h xs)"; auto)
-  apply(cases "l \<le> h \<and> h \<le> length xs"; auto)
-  apply(simp only: SPEC_timerefine_conv)
-  apply(rule SPEC_cong, simp)
-  apply(rule ext)
-  apply(simp add: norm_tr)
-  apply(subst assms(1))
-  apply simp
-  done
-
-  lemma final_insertion_sort2_correct_flexible: 
-    assumes a[simplified, simp]: "(xs',xs)\<in>Id" "(l',l)\<in>Id" "(h',h)\<in>Id"     
-      and tr: "TR ''slice_sort'' = (enat (h-l+1)) *m cost ''call'' 1"
-    shows "final_insertion_sort2 xs' l' h' \<le> \<Down>Id (timerefine TR (final_sort_spec xs l h))"
-    apply(subst fl[where TR=TR, OF tr])
-    apply(rule final_insertion_sort2_correct)
-      apply (fact assms)+
-    oops
-
-  (*
-  proof (simp,rule le_nofailI)
-    assume "nofail (final_sort_spec xs l h)"
-    hence PS: "part_sorted_wrt (le_by_lt (\<^bold><)) is_threshold (slice l h xs)"
-      and LB: "h-l>1" "h \<le> length xs"
-      unfolding final_sort_spec_def slice_sort_spec_def by (auto simp add: refine_pw_simps)
-  
-    from LB have LENGT1: "1 < length (slice l h xs)" by auto
-      
-    
-    have SLR: "(xs, slice l h xs) \<in> slicep_rel l h" using LB
-      by (auto simp: slicep_rel_def)
-    
-    note final_insertion_sort2_refine[OF SLR]
-    also note final_insertion_sort_correct[OF PS LENGT1]
-    also note slice_sort_spec_refine_sort'_sym[OF SLR refl refl refl] 
-    also have "slice_sort_spec (\<^bold><) xs l h \<le> final_sort_spec xs l h"
-      unfolding final_sort_spec_def using PS LB by simp
-    finally show "final_insertion_sort2 xs l h \<le> final_sort_spec xs l h" .
-  qed
-  *)
   
 end
 
 
+subsection \<open>final_insertion_sort3\<close>
 
 context sort_impl_context begin
 
@@ -573,29 +536,32 @@ context sort_impl_context begin
     lxs \<leftarrow> SPECc2 ''sub'' (-) h l;
     if\<^sub>N SPECc2 ''icmp_sle'' (\<le>) lxs is_threshold then do {
       l' \<leftarrow> SPECc2 ''add'' (+) l 1;
-      gen_insertion_sort_guarded3 l l' h xs
+      insertion_sort_guarded3 l l' h xs
     }
     else doN {
       l' \<leftarrow> SPECc2 ''add'' (+) l 1;
       l'' \<leftarrow> SPECc2 ''add'' (+) l is_threshold;
-      xs \<leftarrow> gen_insertion_sort_guarded3 l l' l'' xs;
-      gen_insertion_sort_unguarded3 is_threshold l'' h xs
+      xs \<leftarrow> insertion_sort_guarded3 l l' l'' xs;
+      insertion_sort_unguarded3 is_threshold l'' h xs
     }
   }"  
 
-  thm gen_insertion_sort_unguarded3_refines
+
+subsubsection \<open>Refinement Lemma\<close>
+
   lemma final_insertion_sort3_refines:
     "(xs,xs')\<in>Id \<Longrightarrow> (l,l')\<in>Id \<Longrightarrow> (h,h')\<in>Id 
       \<Longrightarrow> final_insertion_sort3 xs l h \<le> \<Down>Id (timerefine TR_cmp_swap (final_insertion_sort2 xs' l' h'))"
     supply conc_Id[simp del]
     unfolding final_insertion_sort3_def final_insertion_sort2_def
-    supply [refine] = gen_insertion_sort_unguarded3_refines gen_insertion_sort_guarded3_refines
+    supply [refine] = insertion_sort_unguarded3_refines insertion_sort_guarded3_refines
     apply(refine_rcg MIf_refine SPECc2_refine' bindT_refine_conc_time_my_inres monadic_WHILEIT_refine' )
     apply refine_dref_type
     apply(all \<open>(intro  preserves_curr_other_updI wfR''_upd wfR''_TId preserves_curr_TId)?\<close>)
     apply (simp_all (no_asm))
     by auto 
 
+subsubsection \<open>Synthesize final_insertion_sort_impl\<close>
  
   sepref_register final_insertion_sort3  
   sepref_def final_insertion_sort_impl is "uncurry2 (PR_CONST final_insertion_sort3)" 
@@ -606,39 +572,5 @@ context sort_impl_context begin
  
 
 end 
-(*
-context parameterized_weak_ordering begin  
-  definition "final_insertion_sort_param cparam xs l h \<equiv> doN {
-    ASSERT (l<h);
-    if h-l \<le> is_threshold then
-      gen_insertion_sort_param True cparam l (l+1) h xs
-    else doN {
-      xs \<leftarrow> gen_insertion_sort_param True cparam l (l+1) (l+is_threshold) xs;
-      gen_insertion_sort_param False cparam l (l+is_threshold) h xs
-    }
-  }"  
-
-  lemma final_insertion_sort_param_refine[refine]: "\<lbrakk>
-    (l',l)\<in>Id; (h',h)\<in>Id; (xs',xs)\<in>cdom_list_rel cparam
-  \<rbrakk> \<Longrightarrow> final_insertion_sort_param cparam xs' l' h' 
-    \<le> \<Down>(cdom_list_rel cparam) (WO.final_insertion_sort2 cparam xs l h)"  
-    unfolding final_insertion_sort_param_def WO.final_insertion_sort2_def
-    apply refine_rcg
-    apply auto
-    done
-  
-end
-
-context parameterized_sort_impl_context begin
-
-  sepref_register final_insertion_sort_param
-  sepref_def final_insertion_sort_param_impl is "uncurry3 (PR_CONST final_insertion_sort_param)" 
-    :: "cparam_assn\<^sup>k *\<^sub>a wo_assn\<^sup>d *\<^sub>a size_assn\<^sup>k *\<^sub>a size_assn\<^sup>k \<rightarrow>\<^sub>a wo_assn"
-    unfolding final_insertion_sort_param_def PR_CONST_def
-    apply (annot_snat_const "TYPE(size_t)")
-    by sepref
-
-end
-*)
 
 end
