thys/examples/sorting/Sorting_Introsort.thy
@@ -5,14 +5,22 @@ imports
    "Imperative_HOL_Time.Asymptotics_1D"
    "HOL-Real_Asymp.Real_Asymp"
   Sorting_Quicksort_Partition
- (* Sorting_Strings *)
 begin
 
+(* by Manuel Eberl *)
+lemma dlog[asym_bound]:  "(\<lambda>x. real (Discrete.log x)) \<in> \<Theta>(\<lambda>x. ln (real x))"
+proof -
+  have "(\<lambda>x. real (Discrete.log x))  \<in> \<Theta>(\<lambda>n. real (nat \<lfloor>log 2 (real n)\<rfloor>))"
+    by (intro bigthetaI_cong eventually_mono[OF eventually_gt_at_top[of 0]])
+       (auto simp: Discrete.log_altdef)
+  also have "(\<lambda>n. real (nat \<lfloor>log 2 (real n)\<rfloor>)) \<in> \<Theta>(\<lambda>x. ln (real x))"
+    by real_asymp
+  finally show ?thesis .
+qed
 
-
-lemma wfR''_Rsd_a[simp]: "wfR'' (Rsd_a x)"
-  unfolding Rsd_a_def by auto
 context weak_ordering begin
+
+subsection \<open>introsort_aux4 -- using heapsort and partitioner\<close>
 
 
   (* Assemble an introsort loop, using the partitioner and heap-sort *)  
@@ -37,28 +45,20 @@ context weak_ordering begin
   }) (xs,l,h,d)"
 
 
-  definition heapsort_time' :: "_  \<Rightarrow> ecost" where
-    "heapsort_time' s = lift_acost (heapsort_lbc (s)) 
-          + cost ''add'' 1 + cost ''call'' (enat (s) + 2)
-          + cost ''icmp_slt'' (enat (s) + 1 + 1 + 1) + cost ''if'' (enat (s) + 1 + 3)
-          + cost ''sub'' (enat (s) + 2) + cost ''sift_down'' (enat (s))"
+definition "introsort_aux4d xs hml l h \<equiv>
+  doN {
+    loghml \<leftarrow> mop_call (SPECT [Discrete.log hml \<mapsto> log2_iter_cost hml]);
+    d \<leftarrow> SPECc2 ''mul'' (*) loghml 2;
+    introsort_aux4 xs l h d
+  }"
 
-  
-lemma heapsort_correct_h:
-  fixes xs\<^sub>0 :: "'a list"
-    assumes "l\<le>h\<^sub>0" "h\<^sub>0\<le>length xs\<^sub>0"
-    shows "heapsort xs\<^sub>0 l h\<^sub>0 \<le> SPEC (\<lambda>xs. slice_eq_mset l h\<^sub>0 xs xs\<^sub>0 \<and> sorted_wrt_lt (\<^bold><) (slice l h\<^sub>0 xs)) (\<lambda>_. heapsort_time' (h\<^sub>0-l))"
-  apply(rule order.trans[OF heapsort_correct[OF assms]])
-  apply(rule SPEC_leq_SPEC_I) apply simp
-  apply(auto simp: heapsort_time_def heapsort_time'_def heapsort_lbc_def lift_acost_propagate
-        lift_acost_cost)
-  apply sc_solve
-  apply safe by auto
 
 
   
 
 thm heapsort_correct' partition_pivot_correct
+
+subsubsection \<open>Assemble Exchange rate\<close>
 
 text \<open>Here we assemble a Timerefinement from @{term heapsort_TR} and @{term TR_pp}.\<close>
 
@@ -96,29 +96,30 @@ lemma pcTia43[simp]:
   by(auto simp: Tia43_def preserves_curr_def cost_n_eq_TId_n) 
 
 
+subsubsection \<open>Prepare Heapsort\<close>
+
+paragraph \<open>Upper bound cost for heap sort\<close>
+
+text \<open>rules to upperbound hs\<close>
 lemma 
   assumes "1 \<le> Discrete.log (h - l)" "1 \<le> h - l"
   shows 
-    yeah_aux1: "x \<le> y \<Longrightarrow> (h - l) + x \<le> (h - l) * Discrete.log (h - l) + y"
-  and  yeah_aux2: "x \<le> y \<Longrightarrow> p * (h - l) + x \<le> p * (h - l) * Discrete.log (h - l) + y"
-  and  yeah_aux3: "x \<le> y \<Longrightarrow> (h - (1+l)) + x \<le> (h - l) * Discrete.log (h - l) + y"
-  and  yeah_aux4: "x \<le> y \<Longrightarrow> p>0 \<Longrightarrow> p * (h - (1+l)) + x \<le> p * (h - l) * Discrete.log (h - l) + y"
-  and  yeah_aux5: "x \<le> y \<Longrightarrow> (Discrete.log (h - l) * (h - (1+l))) + x \<le> (h - l) * Discrete.log (h - l) + y"
-  and  yeah_aux6: "x \<le> y \<Longrightarrow> p>0 \<Longrightarrow> p * (Discrete.log (h - l) * (h - (1+l))) + x \<le> p * (h - l) * Discrete.log (h - l) + y"
-  and  yeah_aux13: "x \<le> y \<Longrightarrow> ((h - l) * Discrete.log (h - l)) + x \<le> (h - l) * Discrete.log (h - l) + y"
-  and  yeah_aux14: "x \<le> y \<Longrightarrow> p>0 \<Longrightarrow> p * ((h - l) * Discrete.log (h - l)) + x \<le> p * (h - l) * Discrete.log (h - l) + y"
-  and  yeah_aux15: "x \<le> y \<Longrightarrow> p>0 \<Longrightarrow> (h - l) * (p *  Discrete.log (h - l)) + x \<le> p * (h - l) * Discrete.log (h - l) + y"
-  and  yeah_aux7: "x \<le> y \<Longrightarrow> ((h - (1+l)) * Discrete.log (h - l)) + x \<le> (h - l) * Discrete.log (h - l) + y"
-  and  yeah_aux8: "x \<le> y \<Longrightarrow> p>0 \<Longrightarrow> p * ((h - (1+l)) * Discrete.log (h - l)) + x \<le> p * (h - l) * Discrete.log (h - l) + y"
-  and  yeah_aux9: "x \<le> y \<Longrightarrow> (Discrete.log (h - l)) + x \<le> (h - l) * Discrete.log (h - l) + y"
-  and  yeah_aux10: "x \<le> y \<Longrightarrow> p>0 \<Longrightarrow> p * ( Discrete.log (h - l)) + x \<le> p * (h - l) * Discrete.log (h - l) + y"
-  and  yeah_aux11: "x \<le> y \<Longrightarrow> p>0 \<Longrightarrow>(h - (1+l)) * ( p * Discrete.log (h - l)) + x \<le> p * (h - l) * Discrete.log (h - l) + y"
-  and  yeah_aux12: "x \<le> y \<Longrightarrow> p>0 \<Longrightarrow>(h - l) * ( p * Discrete.log (h - l)) + x \<le> p * (h - l) * Discrete.log (h - l) + y"
-  and  yeah_aux_end: "x \<le> y \<Longrightarrow> q>0 \<Longrightarrow> q + x \<le> q * (h - l) * Discrete.log (h - l) + y"
-  subgoal
-    apply(rule add_mono)
-    subgoal using assms by simp 
-    by simp
+    hsub_aux1: "x \<le> y \<Longrightarrow> (h - l) + x \<le> (h - l) * Discrete.log (h - l) + y"
+  and  hsub_aux3: "x \<le> y \<Longrightarrow> (h - (1+l)) + x \<le> (h - l) * Discrete.log (h - l) + y"
+  and  hsub_aux4: "x \<le> y \<Longrightarrow> p>0 \<Longrightarrow> p * (h - (1+l)) + x \<le> p * (h - l) * Discrete.log (h - l) + y"
+  and  hsub_aux2: "x \<le> y \<Longrightarrow> p * (h - l) + x \<le> p * (h - l) * Discrete.log (h - l) + y"
+  and  hsub_aux5: "x \<le> y \<Longrightarrow> (Discrete.log (h - l) * (h - (1+l))) + x \<le> (h - l) * Discrete.log (h - l) + y"
+  and  hsub_aux6: "x \<le> y \<Longrightarrow> p>0 \<Longrightarrow> p * (Discrete.log (h - l) * (h - (1+l))) + x \<le> p * (h - l) * Discrete.log (h - l) + y"
+  and  hsub_aux13: "x \<le> y \<Longrightarrow> ((h - l) * Discrete.log (h - l)) + x \<le> (h - l) * Discrete.log (h - l) + y"
+  and  hsub_aux14: "x \<le> y \<Longrightarrow> p>0 \<Longrightarrow> p * ((h - l) * Discrete.log (h - l)) + x \<le> p * (h - l) * Discrete.log (h - l) + y"
+  and  hsub_aux15: "x \<le> y \<Longrightarrow> p>0 \<Longrightarrow> (h - l) * (p *  Discrete.log (h - l)) + x \<le> p * (h - l) * Discrete.log (h - l) + y"
+  and  hsub_aux7: "x \<le> y \<Longrightarrow> ((h - (1+l)) * Discrete.log (h - l)) + x \<le> (h - l) * Discrete.log (h - l) + y"
+  and  hsub_aux8: "x \<le> y \<Longrightarrow> p>0 \<Longrightarrow> p * ((h - (1+l)) * Discrete.log (h - l)) + x \<le> p * (h - l) * Discrete.log (h - l) + y"
+  and  hsub_aux9: "x \<le> y \<Longrightarrow> (Discrete.log (h - l)) + x \<le> (h - l) * Discrete.log (h - l) + y"
+  and  hsub_aux10: "x \<le> y \<Longrightarrow> p>0 \<Longrightarrow> p * ( Discrete.log (h - l)) + x \<le> p * (h - l) * Discrete.log (h - l) + y"
+  and  hsub_aux11: "x \<le> y \<Longrightarrow> p>0 \<Longrightarrow>(h - (1+l)) * ( p * Discrete.log (h - l)) + x \<le> p * (h - l) * Discrete.log (h - l) + y"
+  and  hsub_aux12: "x \<le> y \<Longrightarrow> p>0 \<Longrightarrow>(h - l) * ( p * Discrete.log (h - l)) + x \<le> p * (h - l) * Discrete.log (h - l) + y"
+  and  hsub_aux_end: "x \<le> y \<Longrightarrow> q>0 \<Longrightarrow> q + x \<le> q * (h - l) * Discrete.log (h - l) + y"
   subgoal
     apply(rule add_mono)
     subgoal using assms by simp 
@@ -130,79 +131,32 @@ lemma
   subgoal
     apply(rule add_mono)
     subgoal apply simp apply(rule order.trans[where b="h-l"]) apply simp using assms by simp
-    by simp
-  subgoal
-    apply(rule add_mono)
-    subgoal using assms by auto
-    by simp
-  subgoal
-    apply(rule add_mono)
-    subgoal using assms by auto
-    by simp
-  subgoal
-    apply(rule add_mono)
-    subgoal using assms by auto
-    by simp
-  subgoal
-    apply(rule add_mono)
-    subgoal using assms by auto
-    by simp
-  subgoal
-    apply(rule add_mono)
-    subgoal using assms by auto
-    by simp
-  subgoal
-    apply(rule add_mono)
-    subgoal using assms by auto
-    by simp
-  subgoal
-    apply(rule add_mono)
-    subgoal using assms by auto
-    by simp
-  subgoal
-    apply(rule add_mono)
-    subgoal using assms by auto
-    by simp
-  subgoal
-    apply(rule add_mono)
-    subgoal using assms by auto
-    by simp
-  subgoal
-    apply(rule add_mono)
-    subgoal using assms by auto
-    by simp
-  subgoal
-    apply(rule add_mono)
-    subgoal using assms by auto
-    by simp
-  subgoal
-    apply(rule add_mono)
-    subgoal using assms by auto
-    by simp
-  done
+    by simp 
+  using assms
+  by(auto intro!: add_mono) 
 
-definition "STOP = (0::nat)"
-lemma yeah_aux0: "a+(STOP::nat)\<le> b\<Longrightarrow> a \<le> b"
+definition "hsub_STOP = (0::nat)"
+lemma hsub_aux0: "a+(hsub_STOP::nat)\<le> b\<Longrightarrow> a \<le> b"
   by simp
 
-lemma yeah_stop: "STOP \<le> 0"
-  unfolding STOP_def by simp
+lemma hsub_stop: "hsub_STOP \<le> 0"
+  unfolding hsub_STOP_def by simp
 
-lemmas yeah_aux = yeah_aux1 yeah_aux2 yeah_aux3 yeah_aux4 yeah_aux5 yeah_aux6
-      yeah_aux13 yeah_aux14 yeah_aux15
-      yeah_aux7 yeah_aux8
-       yeah_aux9 yeah_aux10 yeah_aux11 yeah_aux12 
-      yeah_aux_end
+lemmas hsub_aux = hsub_aux1 hsub_aux2 hsub_aux3 hsub_aux4 hsub_aux5 hsub_aux6
+      hsub_aux13 hsub_aux14 hsub_aux15
+      hsub_aux7 hsub_aux8
+       hsub_aux9 hsub_aux10 hsub_aux11 hsub_aux12 
+      hsub_aux_end
 
-method yeah_solver uses assms  = (simp only: Suc_eq_plus1_left,
-                    rule yeah_aux0,
+method hsub_solver uses assms  = (simp only: Suc_eq_plus1_left,
+                    rule hsub_aux0,
                     simp only: add.assoc,
                     rule order.trans,
-                    (rule yeah_aux[OF assms])+,
-                    rule yeah_stop,
+                    (rule hsub_aux[OF assms])+,
+                    rule hsub_stop,
                     (simp_all, linarith?))
 
-lemma yeah:
+lemma upperbound_heapsort_cost':
   assumes "Discrete.log (h - l) \<ge> 1" "h-l \<ge> 1"
   shows 
   "timerefineA (heapsort_TR l h)  (cost ''slice_sort'' 1)
@@ -225,121 +179,43 @@ lemma yeah:
   apply safe
   subgoal (*if*)  apply(simp add: add_mult_distrib2 add_mult_distrib 
               sc_solve_debug_def numeral_eq_enat plus_enat_simps one_enat_def times_enat_simps) 
-    apply(simp only: Suc_eq_plus1_left)
-    apply(rule yeah_aux0)
-    apply(simp only: add.assoc)
-    apply(rule order.trans)
-     apply(rule yeah_aux[OF assms])+
-        apply(rule yeah_stop)
-    by (simp_all, linarith?)
+    by(hsub_solver assms: assms)
   subgoal (*call*) apply(simp add: add_mult_distrib2 add_mult_distrib 
-              sc_solve_debug_def  numeral_eq_enat plus_enat_simps one_enat_def times_enat_simps) 
-    apply(simp only: Suc_eq_plus1_left)
-    apply(rule yeah_aux0)
-    apply(simp only: add.assoc)
-    apply(rule order.trans)
-     apply(rule yeah_aux[OF assms])+
-        apply(rule yeah_stop)
-    by (simp_all, linarith?)
+              sc_solve_debug_def  numeral_eq_enat plus_enat_simps one_enat_def times_enat_simps)  
+    by(hsub_solver assms: assms)
   subgoal (* sub *) apply(simp add: add_mult_distrib2 add_mult_distrib 
-              sc_solve_debug_def  numeral_eq_enat plus_enat_simps one_enat_def times_enat_simps) 
-    apply(simp only: Suc_eq_plus1_left)
-    apply(rule yeah_aux0)
-    apply(simp only: add.assoc)
-    apply(rule order.trans)
-     apply(rule yeah_aux[OF assms])+
-        apply(rule yeah_stop)
-    by (simp_all, linarith?)
+              sc_solve_debug_def  numeral_eq_enat plus_enat_simps one_enat_def times_enat_simps)  
+    by(hsub_solver assms: assms)
   subgoal (* ''ofs_ptr'' *) apply(simp add: add_mult_distrib2 add_mult_distrib  add.assoc
-              sc_solve_debug_def  numeral_eq_enat plus_enat_simps one_enat_def times_enat_simps) 
-    apply(simp only: Suc_eq_plus1_left)
-    apply(rule yeah_aux0)
-    apply(simp only: add.assoc)
-    apply(rule order.trans)
-     apply(rule yeah_aux[OF assms])+
-        apply(rule yeah_stop)
-    by (simp_all, linarith?)
+              sc_solve_debug_def  numeral_eq_enat plus_enat_simps one_enat_def times_enat_simps)  
+    by(hsub_solver assms: assms)
   subgoal (* ''mul'' *) apply(simp add: add_mult_distrib2 add_mult_distrib  add.assoc
-              sc_solve_debug_def  numeral_eq_enat plus_enat_simps one_enat_def times_enat_simps) 
-    apply(simp only: Suc_eq_plus1_left)
-    apply(rule yeah_aux0)
-    apply(simp only: add.assoc)
-    apply(rule order.trans)
-     apply(rule yeah_aux[OF assms])+
-        apply(rule yeah_stop)
-    by (simp_all, linarith?)
+              sc_solve_debug_def  numeral_eq_enat plus_enat_simps one_enat_def times_enat_simps)  
+    by(hsub_solver assms: assms)
   subgoal (* ''cmpo_v_idx'' *) apply(simp add: add_mult_distrib2 add_mult_distrib  add.assoc
-              sc_solve_debug_def  numeral_eq_enat plus_enat_simps one_enat_def times_enat_simps) 
-    apply(simp only: Suc_eq_plus1_left)
-    apply(rule yeah_aux0)
-    apply(simp only: add.assoc)
-    apply(rule order.trans)
-     apply(rule yeah_aux[OF assms])+
-        apply(rule yeah_stop)
-    by (simp_all, linarith?)
+              sc_solve_debug_def  numeral_eq_enat plus_enat_simps one_enat_def times_enat_simps)  
+    by(hsub_solver assms: assms)
   subgoal (* ''add'' *) apply(simp add: add_mult_distrib2 add_mult_distrib  add.assoc
-              sc_solve_debug_def  numeral_eq_enat plus_enat_simps one_enat_def times_enat_simps) 
-    apply(simp only: Suc_eq_plus1_left)
-    apply(rule yeah_aux0)
-    apply(simp only: add.assoc)
-    apply(rule order.trans)
-     apply(rule yeah_aux[OF assms])+
-        apply(rule yeah_stop)
-    by (simp_all, linarith?)
+              sc_solve_debug_def  numeral_eq_enat plus_enat_simps one_enat_def times_enat_simps)  
+    by(hsub_solver assms: assms)
   subgoal (* ''cmpo_idxs'' *) apply(simp add: add_mult_distrib2 add_mult_distrib  add.assoc
-              sc_solve_debug_def  numeral_eq_enat plus_enat_simps one_enat_def times_enat_simps) 
-    apply(simp only: Suc_eq_plus1_left)
-    apply(rule yeah_aux0)
-    apply(simp only: add.assoc)
-    apply(rule order.trans)
-     apply(rule yeah_aux[OF assms])+
-        apply(rule yeah_stop)
-    by (simp_all, linarith?)
+              sc_solve_debug_def  numeral_eq_enat plus_enat_simps one_enat_def times_enat_simps)  
+    by(hsub_solver assms: assms)
   subgoal (* ''udiv'' *) apply(simp add: add_mult_distrib2 add_mult_distrib  add.assoc
-              sc_solve_debug_def  numeral_eq_enat plus_enat_simps one_enat_def times_enat_simps) 
-    apply(simp only: Suc_eq_plus1_left)
-    apply(rule yeah_aux0)
-    apply(simp only: add.assoc)
-    apply(rule order.trans)
-     apply(rule yeah_aux[OF assms])+
-        apply(rule yeah_stop)
-    by (simp_all, linarith?)
+              sc_solve_debug_def  numeral_eq_enat plus_enat_simps one_enat_def times_enat_simps)  
+    by(hsub_solver assms: assms)
   subgoal (* ''icmp_slt'' *) apply(simp add: add_mult_distrib2 add_mult_distrib  add.assoc
-              sc_solve_debug_def  numeral_eq_enat plus_enat_simps one_enat_def times_enat_simps) 
-    apply(simp only: Suc_eq_plus1_left)
-    apply(rule yeah_aux0)
-    apply(simp only: add.assoc)
-    apply(rule order.trans)
-     apply(rule yeah_aux[OF assms])+
-        apply(rule yeah_stop)
-    by (simp_all, linarith?)
+              sc_solve_debug_def  numeral_eq_enat plus_enat_simps one_enat_def times_enat_simps)  
+    by(hsub_solver assms: assms)
   subgoal (* ''and'' *) apply(simp add: add_mult_distrib2 add_mult_distrib  add.assoc
-              sc_solve_debug_def  numeral_eq_enat plus_enat_simps one_enat_def times_enat_simps) 
-    apply(simp only: Suc_eq_plus1_left)
-    apply(rule yeah_aux0)
-    apply(simp only: add.assoc)
-    apply(rule order.trans)
-     apply(rule yeah_aux[OF assms])+
-        apply(rule yeah_stop)
-    by (simp_all, linarith?)
+              sc_solve_debug_def  numeral_eq_enat plus_enat_simps one_enat_def times_enat_simps)  
+    by(hsub_solver assms: assms)
   subgoal (* ''store'' *) apply(simp add: add_mult_distrib2 add_mult_distrib  add.assoc
-              sc_solve_debug_def  numeral_eq_enat plus_enat_simps one_enat_def times_enat_simps) 
-    apply(simp only: Suc_eq_plus1_left)
-    apply(rule yeah_aux0)
-    apply(simp only: add.assoc)
-    apply(rule order.trans)
-     apply(rule yeah_aux[OF assms])+
-        apply(rule yeah_stop)
-    by (simp_all, linarith?)
+              sc_solve_debug_def  numeral_eq_enat plus_enat_simps one_enat_def times_enat_simps)  
+    by(hsub_solver assms: assms)
   subgoal (* ''load'' *) apply(simp add: add_mult_distrib2 add_mult_distrib  add.assoc
-              sc_solve_debug_def  numeral_eq_enat plus_enat_simps one_enat_def times_enat_simps) 
-    apply(simp only: Suc_eq_plus1_left)
-    apply(rule yeah_aux0)
-    apply(simp only: add.assoc)
-    apply(rule order.trans)
-     apply(rule yeah_aux[OF assms])+
-        apply(rule yeah_stop)
-    by (simp_all, linarith?)
+              sc_solve_debug_def  numeral_eq_enat plus_enat_simps one_enat_def times_enat_simps)  
+    by(hsub_solver assms: assms)
   subgoal (* ''list_swap'' *)
       using assms apply(simp add: add_mult_distrib2 add_mult_distrib  add.assoc
               sc_solve_debug_def  numeral_eq_enat plus_enat_simps one_enat_def times_enat_simps) 
@@ -347,15 +223,16 @@ lemma yeah:
   done
    
   
-lemma yeah': (* i guess h-l must be \<ge> 2 *)
+lemma upperbound_heapsort_cost: (* i guess h-l must be \<ge> 2 *)
   shows 
   "(h-l)>1 \<Longrightarrow> timerefineA (heapsort_TR l h)  (cost ''slice_sort'' 1)
       \<le> timerefineA (Tia43)
        (cost ''slice_sort_p'' (enat ((h-l) * Discrete.log (h-l))))"
-  apply(rule yeah)
+  apply(rule upperbound_heapsort_cost')
   apply auto  
   using Discrete.log.simps by auto  
 
+paragraph \<open>Prepare correctness theorem\<close>
 
 lemma heapsort_correct'': 
   "\<lbrakk>(xs,xs')\<in>Id; (l,l')\<in>Id; (h,h')\<in>Id; lxs=(h'-l'); h'-l'>1\<rbrakk> \<Longrightarrow> heapsort2 xs l h \<le>
@@ -367,11 +244,11 @@ lemma heapsort_correct'':
   apply(simp add: SPEC_timerefine_conv)
   apply(rule SPEC_leq_SPEC_I)
    apply simp 
-  apply(rule yeah') apply simp
+  apply(rule upperbound_heapsort_cost) apply simp
   done 
 
+subsubsection \<open>Prepare Partition Algorithm\<close>
 
-thm partition_pivot_correct_flexible 
 lemma partition_pivot_correct':
   "\<lbrakk>(xs,xs')\<in>Id; (l,l')\<in>Id; (h,h')\<in>Id\<rbrakk> 
   \<Longrightarrow> partition_pivot xs l h \<le> \<Down>Id (timerefine (Tia43) (partition3_spec xs' l' h'))"
@@ -380,22 +257,29 @@ lemma partition_pivot_correct':
   apply (auto )
   done
 
+subsubsection \<open>Refinement Lemma for introsort_aux4\<close>
 
-  lemma introsort_aux4_refine: "introsort_aux4 xs l h d \<le> \<Down>Id (timerefine (Tia43) ((introsort_aux3 (\<lambda>n. n * Discrete.log n) xs l h d)))"
-    unfolding introsort_aux4_def introsort_aux3_def 
-    supply conc_Id[simp del]
-    supply [refine] = mop_call_refine
-    apply (refine_rcg RECT'_refine_t bindT_refine_conc_time_my_inres SPECc2_refine' SPECc2_refine MIf_refine
-            heapsort_correct'' partition_pivot_correct')
-    apply refine_mono
-    apply refine_dref_type
-    apply (simp_all add: inres_SPECc2) 
-    apply(auto simp: Tia43_def )
-    done
+lemma introsort_aux4_refine:
+    "introsort_aux4 xs l h d
+         \<le> \<Down>Id (timerefine (Tia43) ((introsort_aux3 (\<lambda>n. n * Discrete.log n) xs l h d)))"
+  unfolding introsort_aux4_def introsort_aux3_def 
+  supply conc_Id[simp del]
+  supply [refine] = mop_call_refine
+  apply (refine_rcg RECT'_refine_t bindT_refine_conc_time_my_inres SPECc2_refine' SPECc2_refine MIf_refine
+          heapsort_correct'' partition_pivot_correct')
+  apply refine_mono
+  apply refine_dref_type
+  apply (simp_all add: inres_SPECc2) 
+  apply(auto simp: Tia43_def )
+  done
 
 lemma nlogn_mono:
   "\<And>x y. x \<le> y \<Longrightarrow> x * Discrete.log x \<le> y * Discrete.log y"
-    apply(rule mult_mono) apply simp apply (rule log_mono[THEN monoD]) apply simp apply simp apply simp done
+  apply(rule mult_mono)
+     apply simp
+    apply (rule log_mono[THEN monoD])
+  by simp_all
+
 lemma nlogn_sums: 
   "a + b \<le> c \<Longrightarrow> a * Discrete.log a + b * Discrete.log b \<le> c * Discrete.log c"
   apply(rule order.trans)
@@ -404,34 +288,34 @@ lemma nlogn_sums:
   subgoal using log_mono[THEN monoD] by simp
   apply(subst add_mult_distrib[symmetric])
   by simp
+
 lemma nlogn_superlinear: 
   "a * Discrete.log a + b * Discrete.log b \<le> (a+b) * Discrete.log (a+b)"
   apply(rule nlogn_sums) by simp
  
 thm introsort_aux3_correct 
 
-definition "bla d lxs = (pp (pp Tia43 (TId(''list_append'' := 0, ''list_length'' := cost ''sub'' 1))) (TId(''slice_part_sorted'' := introsort_aux_cost (\<lambda>n. n * Discrete.log n) (lxs, d))))"
-
-lemma "bla d lxs = gg"
-  unfolding bla_def 
-  apply(simp add: pp_fun_upd pp_TId_absorbs_right)
-  oops
+definition "E_isa4 d lxs = (pp (pp Tia43 (TId(''list_append'' := 0, ''list_length'' := cost ''sub'' 1)))
+             (TId(''slice_part_sorted'' := introsort_aux_cost (\<lambda>n. n * Discrete.log n) (lxs, d))))"
 
 
-    definition "slice_part_sorted_specT T xsi l h \<equiv> doN { ASSERT (l<h \<and> h\<le>length xsi); SPEC (\<lambda>xsi'. 
-        eq_outside_range xsi' xsi l h 
-      \<and> mset (slice l h xsi') = mset (slice l h xsi) 
-      \<and> part_sorted_wrt (le_by_lt (\<^bold><)) is_threshold (slice l h xsi')) (\<lambda>_. T)}"
+lemma sp_E_isa4[simp]:
+  "struct_preserving (E_isa4 d hl)"
+  unfolding E_isa4_def
+  by (auto simp: pp_fun_upd pp_TId_absorbs_right intro!: struct_preserving_upd_I)  
+
+lemma pc_E_isa4[simp]:
+  "preserves_curr (E_isa4 d hl) ''sub''"
+  "preserves_curr (E_isa4 d hl) ''icmp_slt''"
+  unfolding E_isa4_def
+  by(auto simp: pcTia43[unfolded preserves_curr_def] pp_fun_upd pp_TId_absorbs_right
+                preserves_curr_def cost_n_eq_TId_n) 
+
+
     
-lemma spss1: "slice_part_sorted_spec xs l h = slice_part_sorted_specT (cost ''slice_part_sorted'' 1) xs l h"
-  unfolding slice_part_sorted_specT_def slice_part_sorted_spec_def by auto
+subsubsection \<open>Correctness Lemma for introsort_aux4\<close>
 
-lemma spss2: "timerefine R (slice_part_sorted_specT T xs l h) = slice_part_sorted_specT (timerefineA R T) xs l h"
-  unfolding slice_part_sorted_specT_def 
-  by(cases "l < h \<and> h \<le> length xs", auto simp add: SPEC_timerefine_conv)
-    
-
-lemma introsort_aux4_correct: "introsort_aux4 xs l h d \<le> \<Down> Id (timerefine (bla d (h-l)) (slice_part_sorted_spec xs l h))"
+lemma introsort_aux4_correct: "introsort_aux4 xs l h d \<le> \<Down> Id (timerefine (E_isa4 d (h-l)) (slice_part_sorted_spec xs l h))"
   apply(rule order.trans)
    apply(rule introsort_aux4_refine)
   apply(rule order.trans)
@@ -446,66 +330,53 @@ lemma introsort_aux4_correct: "introsort_aux4 xs l h d \<le> \<Down> Id (timeref
     apply(intro wfR''_upd)
     by simp
   subgoal by auto
-  unfolding bla_def apply simp
+  unfolding E_isa4_def apply simp
   done
 
-definition (in -) "Padad a b = (a=b)"
+definition (in -) "norm_cost_tag a b = (a=b)"
 
-lemma (in -) PadadI: "Padad a a"
-  unfolding Padad_def
+lemma (in -) norm_cost_tagI: "norm_cost_tag a a"
+  unfolding norm_cost_tag_def
   by simp
 
 
-schematic_goal L: "bla d lxs ''slice_part_sorted'' = ?G"
-  unfolding Padad_def[symmetric]
-  unfolding bla_def  
+schematic_goal introsort_aux4_cost_for_slice_part_sorted: "E_isa4 d lxs ''slice_part_sorted'' = ?G"
+  unfolding norm_cost_tag_def[symmetric]
+  unfolding E_isa4_def  
   apply(simp add: norm_cost norm_pp)
-  apply(rule PadadI)
+  apply(rule norm_cost_tagI)
   done
 
-definition "bla2 lxs = (TId(''slice_part_sorted'' := log2_iter_cost lxs + cost ''call'' 1 + cost ''mul'' 1 + bla (Discrete.log lxs * 2) lxs ''slice_part_sorted''))"
 
-definition "introsort_aux4d xs hml l h \<equiv>
-  doN {
-    loghml \<leftarrow> mop_call (SPECT [Discrete.log hml \<mapsto> log2_iter_cost hml]);
-    d \<leftarrow> SPECc2 ''mul'' (*) loghml 2;
-    introsort_aux4 xs l h d
-  }"
+subsubsection \<open>Correctness Lemma for introsort_aux4d\<close>
 
-lemma "timerefineA (bla2 hml) (cost ''slice_part_sorted'' 1)
-        = G" unfolding bla2_def Tia43_def apply(simp add: norm_cost norm_pp) oops
-
-lemma gwp_SPECc2:
-  assumes "Some (t + cost c 1) \<le> Q (op a b)"
-  shows "Some t \<le> gwp (SPECc2 c op a b) Q"
-  unfolding SPECc2_def 
-  apply(refine_vcg \<open>-\<close>)
-  using assms by auto
+definition "E_isa4d lxs = (TId(''slice_part_sorted'' := log2_iter_cost lxs + cost ''call'' 1 
+                       + cost ''mul'' 1 + E_isa4 (Discrete.log lxs * 2) lxs ''slice_part_sorted''))"
 
 
 
-lemma le_acost_ASSERTI_otherdir:
-  fixes M :: "(_,(_,enat) acost) nrest"
-  shows "M \<le> ASSERT \<Phi> \<bind> (\<lambda>_. M') \<Longrightarrow> (\<Phi> \<Longrightarrow> M \<le> M')"
-  by(auto simp: pw_acost_le_iff refine_pw_simps)
-
-lemma introsort_aux4d_correct: "hml = h-l \<Longrightarrow> introsort_aux4d xs hml l h \<le> \<Down> Id (timerefine (bla2 hml) (slice_part_sorted_spec xs l h))"
+lemma introsort_aux4d_correct:
+  assumes "hml = h-l"
+  shows "introsort_aux4d xs hml l h
+           \<le> \<Down> Id (timerefine (E_isa4d hml) (slice_part_sorted_spec xs l h))"
+  using assms
   unfolding introsort_aux4d_def
-  unfolding spss1 spss2 
+  unfolding spss_eq1 spss_eq2 
   apply simp
   unfolding slice_part_sorted_specT_def
   apply(cases "l < h \<and> h \<le> length xs", auto)
   unfolding SPEC_REST_emb'_conv
   apply(rule gwp_specifies_I)
-  supply insort4 = introsort_aux4_correct[unfolded spss1 spss2, unfolded slice_part_sorted_specT_def SPEC_REST_emb'_conv, simplified,
+  supply insort4 = introsort_aux4_correct[unfolded spss_eq1 spss_eq2, unfolded slice_part_sorted_specT_def SPEC_REST_emb'_conv, simplified,
           THEN le_acost_ASSERTI_otherdir, THEN gwp_specifies_rev_I, THEN gwp_conseq_0]
   apply(refine_vcg \<open>-\<close> rules: gwp_SPECc2 insort4)
    apply(auto simp: Some_eq_emb'_conv emb_le_Some_conv )
-  by(simp add: bla2_def norm_cost add.left_commute add.commute add.assoc)
+  by(simp add: E_isa4d_def norm_cost add.left_commute add.commute add.assoc)
 
 lemma TR_sps_important2:
-  assumes "TR ''slice_part_sorted'' = bla2 (h - l) ''slice_part_sorted''"
-  shows "timerefine TR (slice_part_sorted_spec xs l h) = (timerefine (bla2 (h-l)) (slice_part_sorted_spec xs l h))"
+  assumes "TR ''slice_part_sorted'' = E_isa4d (h - l) ''slice_part_sorted''"
+  shows "timerefine TR (slice_part_sorted_spec xs l h)
+             = (timerefine (E_isa4d (h-l)) (slice_part_sorted_spec xs l h))"
   unfolding slice_part_sorted_spec_def
   apply(cases "l < h \<and> h \<le> length xs"; auto)
   apply(simp only: SPEC_timerefine_conv)
@@ -517,7 +388,7 @@ lemma TR_sps_important2:
   done
 
 lemma introsort_aux4d_correct_flexible:
-  assumes "TR ''slice_part_sorted'' = bla2 (h - l) ''slice_part_sorted''"
+  assumes "TR ''slice_part_sorted'' = E_isa4d (h - l) ''slice_part_sorted''"
     and "hml = h-l"
   shows "introsort_aux4d xs hml l h \<le> \<Down> Id (timerefine TR (slice_part_sorted_spec xs l h))"
   apply(subst TR_sps_important2[where TR=TR, OF assms(1)])
@@ -528,6 +399,7 @@ lemma introsort_aux4d_correct_flexible:
 
 
 
+subsection \<open>introsort4\<close>
 
   definition "introsort4 xs l h \<equiv> doN {
     ASSERT(l\<le>h);
@@ -539,30 +411,15 @@ lemma introsort_aux4d_correct_flexible:
     } else RETURN xs
   }"  
 
-lemma wfR''_bla[simp]: " wfR'' (bla d xs)"
-  unfolding bla_def
-  by(auto simp add:  pp_fun_upd pp_TId_absorbs_right intro!: wfR''_upd) 
-
-thm introsort_aux4_correct
-
 lemmas final_insertion_sort2_correct_flexible = final_insertion_sort2_correct
 
-thm introsort_aux4d_correct_flexible
-thm final_insertion_sort2_correct_flexible
-
 abbreviation "TR_is d s == TId(''lt'':=cost ''icmp_slt'' 1,''slice_sort'' := fi2_cost s, 
-            ''slice_part_sorted'':= log2_iter_cost s + cost ''call'' 1 + cost ''mul'' 1 + bla d s ''slice_part_sorted'')"
-
-lemma pc_bla[simp]:
-  "preserves_curr (bla d hl) ''sub''"
-  "preserves_curr (bla d hl) ''icmp_slt''"
-  by(auto simp: pcTia43[unfolded preserves_curr_def] pp_fun_upd pp_TId_absorbs_right  bla_def preserves_curr_def cost_n_eq_TId_n) 
+            ''slice_part_sorted'':= log2_iter_cost s + cost ''call'' 1 + cost ''mul'' 1 + E_isa4 d s ''slice_part_sorted'')"
 
 lemma pc_TR_is[simp]:
   "preserves_curr (TR_is d hl) ''sub''"
   "preserves_curr (TR_is d hl) ''icmp_slt''"
   by(auto simp: preserves_curr_def cost_n_eq_TId_n) 
-
 
 lemma wfR''_TR_is[simp]: "wfR'' (TR_is d hl)"
   by (auto intro!: wfR''_upd)
@@ -572,65 +429,14 @@ lemma sp_TR_is[simp]:
   by (auto intro!: struct_preserving_upd_I) 
 
 
-lemma sp_bla[simp]:
-  "struct_preserving (bla d hl)"
-  by (auto simp: pp_fun_upd pp_TId_absorbs_right  bla_def intro!: struct_preserving_upd_I)  
-
-(*TODO: move*)
-
-lemma SPECc1_alt: "SPECc1 name aop = ( (\<lambda>a. consume (RETURNT (aop a)) (cost name 1)))"
-  unfolding SPECc1_def consume_def by(auto simp: RETURNT_def intro!: ext)
-
-  lemma introsort4_refine: "introsort4 xs l h \<le> \<Down>Id (timerefine (TR_is (Discrete.log (h-l)*2) (h-l)) (introsort3 xs l h))"
-    unfolding introsort4_def introsort3_def 
-    supply conc_Id[simp del]
-    apply (refine_rcg SPECc2_refine' SPECc2_refine bindT_refine_conc_time_my_inres MIf_refine
-                introsort_aux4d_correct_flexible final_insertion_sort2_correct_flexible
-               consumea_refine   )
-    apply refine_dref_type                                          
-   by (auto simp: bla2_def norm_cost inres_SPECc2) 
-
-
-  thm introsort4_refine introsort3_correct
-
-abbreviation "TR_is4 lmh \<equiv> pp (TR_is (Discrete.log (lmh)*2) (lmh)) (TId(''slice_sort'' := introsort3_cost))" 
-
-lemma "introsort4 xs l h \<le> \<Down> Id (timerefine (TR_is4 (h-l)) (slice_sort_spec (\<^bold><) xs l h))"
-  apply(rule order.trans)
-   apply(rule introsort4_refine)
-  apply simp
-      apply(subst timerefine_iter2[symmetric])
-      subgoal by(auto intro!: wfR''_upd)
-      subgoal by(auto simp: norm_pp intro!: wfR''_upd)
-      apply(rule timerefine_mono2)
-      subgoal by(auto intro!: wfR''_upd)
-      apply(rule order.trans)
-      apply(rule introsort3_correct)
-      apply simp
-      done
-
-lemma "\<Down> Id (timerefine (TR_is4 (h-l)) (slice_sort_spec (\<^bold><) xs l h))
-    = slice_sort_specT G (\<^bold><) xs l h"
-  apply(cases "l \<le> h \<and> h \<le> length xs")
-   apply (auto simp: slice_sort_spec_def slice_sort_specT_def SPEC_timerefine_conv )
-  apply(rule SPEC_cong)
-   apply simp
-  apply(rule ext)
-  apply (simp add: norm_cost norm_pp)
-  unfolding introsort3_cost_def bla_def TR_is_insert3_def Tia43_def
-    cost_insert_guarded_def cost_insert_def
-    cost_is_insert_step_def cost_is_insert_guarded_step_def
-    introsort_aux_cost_def
-  apply (simp add: norm_cost norm_pp)
-  apply(subst timerefineA_propagate, intro wfR''_upd wfR''_TId)+
-  apply (simp add: norm_cost norm_pp)
-  unfolding move_median_to_first_cost_def
-  apply (simp add: norm_cost norm_pp)
-  oops
-    
-    
-
-  (* lemmas introsort4_correct = order_trans[OF introsort4_refine introsort3_correct] *)
+lemma introsort4_refine: "introsort4 xs l h \<le> \<Down>Id (timerefine (TR_is (Discrete.log (h-l)*2) (h-l)) (introsort3 xs l h))"
+  unfolding introsort4_def introsort3_def 
+  supply conc_Id[simp del]
+  apply (refine_rcg SPECc2_refine' SPECc2_refine bindT_refine_conc_time_my_inres MIf_refine
+              introsort_aux4d_correct_flexible final_insertion_sort2_correct_flexible
+             consumea_refine   )
+  apply refine_dref_type                                          
+ by (auto simp: E_isa4d_def norm_cost inres_SPECc2) 
 
 end
 
@@ -654,14 +460,7 @@ qed
 
 context sort_impl_context begin
 
-
-thm partition_pivot2_refines heapsort3_refine
-
-
-lemma TR_sup_Tid: "sup TId TId = TId"
-  by simp
-
-
+subsection \<open>introsort_aux5 -- using cmp and swap\<close>
 
   definition introsort_aux5 :: "'a list \<Rightarrow> nat \<Rightarrow> nat \<Rightarrow> nat \<Rightarrow> ('a list, ecost) nrest"
     where "introsort_aux5 xs l h d \<equiv> RECT' (\<lambda>introsort_aux (xs,l,h,d). doN {
@@ -688,6 +487,7 @@ lemma pc_TR_cmp_swap: "x\<noteq>''cmp_idxs'' \<Longrightarrow> x\<noteq>''cmpo_i
   apply(intro preserves_curr_other_updI)
   by auto
 
+subsubsection \<open>refine compare and swap\<close>
 
 lemma introsort_aux5_refine: "(xs,xs')\<in>Id \<Longrightarrow> (l,l')\<in>Id \<Longrightarrow> (h,h')\<in>Id \<Longrightarrow> (d,d')\<in>Id 
     \<Longrightarrow> introsort_aux5 xs l h d \<le> \<Down>Id (timerefine (TR_cmp_swap) ((introsort_aux4 xs' l' h' d')))"
@@ -701,17 +501,19 @@ lemma introsort_aux5_refine: "(xs,xs')\<in>Id \<Longrightarrow> (l,l')\<in>Id \<
     done
 
 
-
-
+subsubsection \<open>synthesize program\<close>
 
 sepref_register introsort_aux5
-sepref_def introsort_aux_impl is "uncurry3 (PR_CONST introsort_aux5)" :: "(arr_assn)\<^sup>d *\<^sub>a size_assn\<^sup>k *\<^sub>a size_assn\<^sup>k *\<^sub>a size_assn\<^sup>k \<rightarrow>\<^sub>a arr_assn"
+sepref_def introsort_aux_impl is
+  "uncurry3 (PR_CONST introsort_aux5)"
+    :: "(arr_assn)\<^sup>d *\<^sub>a size_assn\<^sup>k *\<^sub>a size_assn\<^sup>k *\<^sub>a size_assn\<^sup>k \<rightarrow>\<^sub>a arr_assn"
   unfolding introsort_aux5_def PR_CONST_def
   apply (annot_snat_const "TYPE('size_t)")
   supply [[goals_limit = 1]]
   by sepref
 
 
+subsection \<open>introsort5\<close>
 
 
   definition "introsort5 xs l h \<equiv> doN {
@@ -727,6 +529,7 @@ sepref_def introsort_aux_impl is "uncurry3 (PR_CONST introsort_aux5)" :: "(arr_a
   }"  
 
 
+subsubsection \<open>refine compare and swap\<close>
 
   lemma introsort5_refine: "introsort5 xs l h \<le> \<Down>Id (timerefine (TR_cmp_swap) ((introsort4 xs l h )))"
     unfolding introsort4_def introsort_aux4d_def introsort5_def 
@@ -739,7 +542,6 @@ sepref_def introsort_aux_impl is "uncurry3 (PR_CONST introsort_aux5)" :: "(arr_a
     apply (auto simp add: inres_SPECc2 intro!: pc_TR_cmp_swap) 
     done
  
-  thm sepref_fr_rules
 
 lemma mop_call_same_result:
   fixes m :: "(_,(_,enat) acost)nrest"
@@ -750,8 +552,9 @@ lemma mop_call_same_result:
     by (simp add: ecost_nneg)
   done
 
-lemma AAA: (* TODO: Move depth-computation into own (inline) function *)
-  assumes "hml < max_snat N" "RETURNTecost xb \<le> mop_call (log2_iter hml)" "1<N" shows "xb * 2 < max_snat N"
+lemma introsort5_synth_side_condition: (* TODO: Move depth-computation into own (inline) function *)
+  assumes "hml < max_snat N" "RETURNTecost xb \<le> mop_call (log2_iter hml)" "1<N"
+  shows "xb * 2 < max_snat N"
 proof -
   from order_trans[OF mop_call_same_result[OF assms(2)] log2_iter_refine]
   have xb: "xb = Discrete.log hml"
@@ -765,28 +568,25 @@ proof -
 qed
  
 
+subsubsection \<open>synthesize program\<close>
 
 sepref_register introsort5
-sepref_def introsort_impl is "uncurry2 (PR_CONST introsort5)" :: "(arr_assn)\<^sup>d *\<^sub>a size_assn\<^sup>k *\<^sub>a size_assn\<^sup>k \<rightarrow>\<^sub>a arr_assn"
+sepref_def introsort_impl is 
+  "uncurry2 (PR_CONST introsort5)"
+    :: "(arr_assn)\<^sup>d *\<^sub>a size_assn\<^sup>k *\<^sub>a size_assn\<^sup>k \<rightarrow>\<^sub>a arr_assn"
   unfolding introsort5_def PR_CONST_def
   apply (annot_snat_const "TYPE('size_t)")
-  supply [intro!] = AAA 
+  supply [intro!] = introsort5_synth_side_condition 
   by sepref
 
-  (*
-lemma introsort4_refine_ss_spec: "(PR_CONST introsort4, slice_sort_spec (\<^bold><))\<in>Id\<rightarrow>Id\<rightarrow>Id\<rightarrow>\<langle>Id\<rangle>nres_rel"  
-  using introsort4_correct by (auto intro: nres_relI)
-  
-theorem introsort_impl_correct: "(uncurry2 introsort_impl, uncurry2 (slice_sort_spec (\<^bold><))) \<in> arr_assn\<^sup>d *\<^sub>a snat_assn\<^sup>k *\<^sub>a snat_assn\<^sup>k \<rightarrow>\<^sub>a arr_assn"  
-  using introsort_impl.refine[FCOMP introsort4_refine_ss_spec] .
-  
-  *)
+subsection \<open>Compose the correctness theorems\<close>                                   
 
-                                   
-thm introsort5_refine introsort4_refine introsort3_correct
+text \<open>When composing the correctness theorems of @{term introsort5},
+    @{term introsort4} and @{term introsort3},
+     we synthesize a compound exchange rate ?E:\<close>
 
 schematic_goal introsort5_correct:
-  "introsort5 xs l h \<le> \<Down> Id (timerefine ?TR (slice_sort_spec (\<^bold><) xs l h))"
+  "introsort5 xs l h \<le> \<Down> Id (timerefine ?E (slice_sort_spec (\<^bold><) xs l h))"
   apply(rule order.trans)
   apply(rule introsort5_refine)
   apply (rule nrest_Rel_mono)
@@ -815,11 +615,11 @@ schematic_goal introsort5_correct:
   done 
 
 
-concrete_definition introsort5_TR is introsort5_correct uses "_ \<le> \<Down> Id (timerefine \<hole> _) "
-print_theorems
+text \<open>And give this exchange rate a Name:\<close>
 
-thm introsort5_TR.refine
-lemma argh_foo: "(timerefine (introsort5_TR l h) (slice_sort_spec (\<^bold><) xs l h))
+concrete_definition introsort5_TR is introsort5_correct uses "_ \<le> \<Down> Id (timerefine \<hole> _) "
+
+lemma pull_introsort5_TR_into_spec: "(timerefine (introsort5_TR l h) (slice_sort_spec (\<^bold><) xs l h))
     = slice_sort_specT (introsort5_TR l h ''slice_sort'') (\<^bold><) xs l h"
   unfolding slice_sort_spec_def slice_sort_specT_def
   apply(cases "l \<le> h \<and> h \<le> length xs")
@@ -828,30 +628,15 @@ lemma argh_foo: "(timerefine (introsort5_TR l h) (slice_sort_spec (\<^bold><) xs
   by (auto simp: timerefineA_cost)
 
 
-thm introsort5_TR.refine[unfolded argh]
 
-lemma leq_sc_l_TERMINATE_special:
-  "P \<Longrightarrow> leq_sidecon (cost n x) 0 0 0 0 (cost n x + 0) P"
-   
-  unfolding leq_sidecon_def by (simp add: cost_zero)
-
-lemma leq_sc_l_DONE_special:
-  "leq_sidecon 0 l 0 0 0 (bs3+0) P \<Longrightarrow> leq_sidecon (cost n x) l 0 0 0 ((cost n x + bs3) + 0) P"
-   
-  unfolding leq_sidecon_def apply (simp add: cost_zero)
-  apply(rule add_mono) by auto
-
-lemma leq_sc_l_NEXT_ROW_special:
-  "leq_sidecon (cost n x) 0 ls 0 0 bs P \<Longrightarrow> leq_sidecon 0 ((cost n x)+ls) 0 0 0 bs P"
-  unfolding leq_sidecon_def by (simp add: cost_zero) 
-
+text \<open>We simplify @{term introsort5_TR}\<close>
 
 schematic_goal ub_introsort5: "timerefineA (introsort5_TR l h) (cost ''slice_sort'' 1) \<le> ?x"
   unfolding introsort5_TR_def introsort3_cost_def
   apply(simp add: norm_pp norm_cost )
   apply(subst timerefineA_propagate, (auto intro!: wfR''_upd)[1])+ 
   apply(simp add: norm_pp norm_cost )
-  unfolding log2_iter_cost_def TR_is_insert3_def bla_def Tia43_def introsort_aux_cost_def
+  unfolding log2_iter_cost_def TR_is_insert3_def E_isa4_def Tia43_def introsort_aux_cost_def
       cost_insert_guarded_def cost_is_insert_guarded_step_def
       cost_insert_def cost_is_insert_step_def move_median_to_first_cost_def
   apply(simp add: norm_pp norm_cost )
@@ -864,48 +649,26 @@ schematic_goal ub_introsort5: "timerefineA (introsort5_TR l h) (cost ''slice_sor
   apply(simp add: add.assoc add.commute add.left_commute)
   apply(simp add: cost_same_curr_left_add cost_same_curr_add) 
   apply(simp add: add.assoc add.commute add.left_commute)
-  
-  apply ( (simp only: add.assoc)?; rule leq_sc_init, (simp only: add.assoc)?)
-  apply ( ((rule leq_sc_l_SUCC leq_sc_l_FAIL )+)?,
-            ((rule leq_sc_l_DONE_special, rule leq_sc_l_NEXT_ROW_special)
-              | (rule  leq_sc_l_TERMINATE_special))  )+ 
+
+  apply sc_solve_upperbound
   by simp
 
-
+text \<open>and give it a name\<close>
 concrete_definition introsort5_acost is ub_introsort5 uses "_ \<le> \<hole>"
-print_theorems
 
-schematic_goal iii: "introsort5_acost x y = lift_acost ?y"
+text \<open>we pull the lifting to the outer most:\<close>
+schematic_goal lift_introsort5_acost: "introsort5_acost x y = lift_acost ?y"
   unfolding introsort5_acost_def
   apply(simp add: numeral_eq_enat one_enat_def)
   unfolding lift_acost_cost[symmetric]  lift_acost_propagate[symmetric]
   apply(rule refl)
   done
-concrete_definition introsort5_cost is iii uses "_ = lift_acost \<hole>"
-print_theorems
-  
 
-lemmas introsort_rule' = hn_refine_result[OF introsort_impl.refine[to_hnr], unfolded PR_CONST_def APP_def, OF 
-      introsort5_TR.refine ]
-lemma intro_rule: "hn_refine (hn_ctxt arr_assn a ai \<and>* hn_val snat_rel ba bia \<and>* hn_val snat_rel b bi)
-       (introsort_impl ai bia bi)
-       (hn_invalid arr_assn a ai \<and>* hn_val snat_rel ba bia \<and>* hn_val snat_rel b bi) (hr_comp arr_assn Id)
- (timerefine (introsort5_TR ba b) (slice_sort_spec (\<^bold><) a ba b))"
-  apply(rule introsort_rule')
-  apply(rule attains_sup_sv) by simp
-
-lemmas pff = intro_rule[unfolded slice_sort_spec_def SPEC_REST_emb'_conv,  THEN ht_from_hnr]
-
-thm llvm_htriple_more_time[OF introsort5_acost.refine pff, unfolded introsort5_cost.refine  ]
+text \<open>We define the finite part of the cost expression:\<close>
+concrete_definition introsort5_cost is lift_introsort5_acost uses "_ = lift_acost \<hole>"
 
 
-
-lemma Sum_any_cost2: "Sum_any (the_acost (cost n x)) = x"
-  unfolding cost_def by (simp add: zero_acost_def)
-
-
-thm introsort5_cost_def[no_vars]
-
+text \<open>We display the final cost expression::\<close>
 definition "introsort_cost3 s \<equiv>
 cost ''mul'' (Suc (s * Discrete.log s * 14)) +
 (cost ''ofs_ptr'' (1241 + (108 * (s * Discrete.log s) + 68 * s)) +
@@ -918,171 +681,97 @@ cost ''mul'' (Suc (s * Discrete.log s * 14)) +
        (cost ''and'' (s * Discrete.log s * 6) +
         (cost ''icmp_slt'' (20 + (2 * s + (25 * (s * Discrete.log s) + Discrete.log s))) +
          (cost ''udiv'' (Suc (18 * (s * Discrete.log s) + Discrete.log s)) +
-          (cost ''call'' (343 + (22 * (s * Discrete.log s) + (19 * s + Discrete.log s))) + (cost ''icmp_eq'' (289 + (s + Discrete.log s * 2 * s)) + cost ''icmp_sle'' (Suc 0)))))))))))))" 
+          (cost ''call'' (343 + (22 * (s * Discrete.log s) + (19 * s + Discrete.log s))) +
+           (cost ''icmp_eq'' (289 + (s + Discrete.log s * 2 * s)) +
+             cost ''icmp_sle'' 1))))))))))))" 
  
-lemma 35: "introsort_cost3 (h-l) = introsort5_cost l h" 
+lemma introsort_cost3_eq_introsort_cost5: "introsort_cost3 (h-l) = introsort5_cost l h" 
   unfolding introsort_cost3_def introsort5_cost_def by (auto simp: algebra_simps)
 
+definition "introsort_impl_cost n = lift_acost (introsort_cost3 n)"
 
-lemma final_hoare_triple: "ba \<le> b \<and> b \<le> length a \<Longrightarrow>
-llvm_htriple ($lift_acost (introsort_cost3 (b-ba)) \<and>* hn_ctxt arr_assn a ai \<and>* hn_val snat_rel ba bia \<and>* hn_val snat_rel b bi) (introsort_impl ai bia bi)
- (\<lambda>r. (\<lambda>s. \<exists>x. (\<up>(length x = length a \<and> take ba x = take ba a \<and> drop b x = drop b a \<and> sort_spec (\<^bold><) (slice ba b a) (slice ba b x)) \<and>* hr_comp arr_assn Id x r) s) \<and>*
-      hn_invalid arr_assn a ai \<and>* hn_val snat_rel ba bia \<and>* hn_val snat_rel b bi)"
-  apply(rule llvm_htriple_more_time[OF introsort5_acost.refine pff, unfolded introsort5_cost.refine 35[symmetric] ])
+lemma "introsort_impl_cost (h-l) = introsort5_acost l h"
+  unfolding introsort_impl_cost_def introsort5_cost.refine introsort_cost3_eq_introsort_cost5 
   by simp
+  
+
+text \<open>Combine Refinement lemma for @{term introsort_impl} with correctness theorem\<close>
+
+lemmas introsort_correct' = hn_refine_result[OF introsort_impl.refine[to_hnr],
+                                              unfolded PR_CONST_def APP_def,
+                                              OF introsort5_TR.refine ]
+
+lemma introsort_correct:
+ "hn_refine (hn_ctxt arr_assn a ai \<and>* hn_val snat_rel ba bia \<and>* hn_val snat_rel b bi)
+       (introsort_impl ai bia bi)
+ (hn_invalid arr_assn a ai \<and>* hn_val snat_rel ba bia \<and>* hn_val snat_rel b bi) (hr_comp arr_assn Id)
+  (timerefine (introsort5_TR ba b) (slice_sort_spec (\<^bold><) a ba b))"
+  apply(rule introsort_correct')
+  apply(rule attains_sup_sv) by simp
+
+text \<open>extract Hoare Triple\<close>
+
+lemmas introsort_ht = introsort_correct[unfolded slice_sort_spec_def SPEC_REST_emb'_conv,
+                                          THEN ht_from_hnr]
+
+lemma Sum_any_cost2: "Sum_any (the_acost (cost n x)) = x"
+  unfolding cost_def by (simp add: zero_acost_def)
+
+
+subsection \<open>The final Hoare Triple\<close>
+
+abbreviation "slice_sort_aux xs\<^sub>0 xs l h \<equiv> (length xs = length xs\<^sub>0 \<and> take l xs = take l xs\<^sub>0
+                    \<and> drop h xs = drop h xs\<^sub>0 \<and> sort_spec (\<^bold><) (slice l h xs\<^sub>0) (slice l h xs))"
+
+lemma final_hoare_triple:
+  assumes "l \<le> h \<and> h \<le> length xs\<^sub>0"
+  shows "llvm_htriple ($introsort_impl_cost (h-l) \<and>* hn_ctxt arr_assn xs\<^sub>0 p
+           \<and>* hn_val snat_rel l l' \<and>* hn_val snat_rel h h')
+        (introsort_impl p l' h')
+      (\<lambda>r. (\<lambda>s. \<exists>xs. (\<up>(slice_sort_aux xs\<^sub>0 xs l h) \<and>* hr_comp arr_assn Id xs r) s)
+           \<and>* hn_invalid arr_assn xs\<^sub>0 p \<and>* hn_val snat_rel l l' \<and>* hn_val snat_rel h h')"
+  unfolding introsort_impl_cost_def
+  using assms
+  by (rule llvm_htriple_more_time[OF introsort5_acost.refine introsort_ht,
+                unfolded introsort5_cost.refine introsort_cost3_eq_introsort_cost5[symmetric] ])
+
+
+
+text \<open>Calculate the cost for all currencies:\<close>
 
 schematic_goal Sum_any_calc: "Sum_any (the_acost (introsort_cost3 s)) = ?x"
-  unfolding Padad_def[symmetric]
+  unfolding norm_cost_tag_def[symmetric]
   unfolding introsort_cost3_def 
   apply(simp add: the_acost_propagate add.assoc) 
   apply(subst Sum_any.distrib;  ( auto simp only: Sum_any_cost 
           intro!: finite_sum_nonzero_cost finite_sum_nonzero_if_summands_finite_nonzero))+
-  apply(rule PadadI)
+  apply(rule norm_cost_tagI)
   done
 
+text \<open>Give the result a name:\<close>
+concrete_definition (in -) introsort3_allcost is sort_impl_context.Sum_any_calc uses "_ = \<hole>"
+
+lemma "introsort3_allcost n = Sum_any (the_acost (introsort_cost3 n))"  
+  apply(subst introsort3_allcost.refine[OF sort_impl_context_axioms, symmetric])
+  by simp
 
 end 
 
-(* TODO: there is a problem with auto2 in a context *)
-concrete_definition introsort_cost3_all is sort_impl_context.Sum_any_calc uses "_ = \<hole>"
+text \<open>The cost of introsort expanded:\<close>
 
-lemma "introsort_cost3_all n = 4693 + 5 *  Discrete.log n + 231 * n + 455 * (n * Discrete.log n)"
-  unfolding introsort_cost3_all_def
+lemma "introsort3_allcost n = 4693 + 5 *  Discrete.log n + 231 * n + 455 * (n * Discrete.log n)"
+  unfolding introsort3_allcost_def
   apply (simp add: algebra_simps)
   done
 
-(* by Manuel Eberl *)
-lemma dlog[asym_bound]:  "(\<lambda>x. real (Discrete.log x)) \<in> \<Theta>(\<lambda>x. ln (real x))"
-proof -
-  have "(\<lambda>x. real (Discrete.log x))  \<in> \<Theta>(\<lambda>n. real (nat \<lfloor>log 2 (real n)\<rfloor>))"
-    by (intro bigthetaI_cong eventually_mono[OF eventually_gt_at_top[of 0]])
-       (auto simp: Discrete.log_altdef)
-  also have "(\<lambda>n. real (nat \<lfloor>log 2 (real n)\<rfloor>)) \<in> \<Theta>(\<lambda>x. ln (real x))"
-    by real_asymp
-  finally show ?thesis .
-qed
- 
 
-lemma "(\<lambda>n. real (n* Discrete.log n)) \<in> \<Theta>(\<lambda>n. (real n)* (ln (real n)))"
-  apply auto2
-  done
+text \<open>The asymptotic behaviour of introsort's cost:\<close>
 
-lemma "(\<lambda>x. real (x + Suc (x * 14) + 10) ) \<in> \<Theta>(\<lambda>n. (real n))"
-  unfolding Suc_eq_plus1_left
-  apply simp
-  apply auto2 done
-
-lemma "(\<lambda>x. real (introsort_cost3_all x)) \<in> \<Theta>(\<lambda>n. (real n)*(ln (real n)))"
-  unfolding introsort_cost3_all_def
+lemma "(\<lambda>x. real (introsort3_allcost x)) \<in> \<Theta>(\<lambda>n. (real n)*(ln (real n)))"
+  unfolding introsort3_allcost_def
   unfolding Suc_eq_plus1_left
   apply simp
   by auto2
-
-
-
-(*
-context parameterized_weak_ordering begin
-  (* TODO: Move *)
-  lemmas heapsort_param_refine'[refine] = heapsort_param_refine[unfolded heapsort1.refine[OF WO.weak_ordering_axioms, symmetric]]
-  
-  
-  definition introsort_aux_param :: "'cparam \<Rightarrow> 'a list \<Rightarrow> nat \<Rightarrow> nat \<Rightarrow> nat \<Rightarrow> 'a list nres" where 
-    "introsort_aux_param cparam xs l h d \<equiv> RECT (\<lambda>introsort_aux (xs,l,h,d). doN {
-    ASSERT (l\<le>h);
-    if h-l > is_threshold then doN {
-      if d=0 then
-        heapsort_param cparam xs l h
-      else doN {
-        (xs,m)\<leftarrow>partition_pivot_param cparam xs l h;
-        xs \<leftarrow> introsort_aux (xs,l,m,d-1);
-        xs \<leftarrow> introsort_aux (xs,m,h,d-1);
-        RETURN xs
-      }
-    }
-    else
-      RETURN xs
-  }) (xs,l,h,d)"
-
-
-  lemma introsort_aux_param_refine[refine]: 
-    "\<lbrakk> (xs',xs)\<in>cdom_list_rel cparam; (l',l)\<in>Id; (h',h)\<in>Id; (d',d)\<in>Id
-    \<rbrakk> \<Longrightarrow> introsort_aux_param cparam xs' l' h' d' \<le>\<Down>(cdom_list_rel cparam) (WO.introsort_aux4 cparam xs l h d)"
-    unfolding introsort_aux_param_def WO.introsort_aux4_def 
-    supply [refine_dref_RELATES] = RELATESI[of "cdom_list_rel cparam"]
-    apply (refine_rcg)
-    apply refine_dref_type
-    apply simp_all 
-    done
-
-  definition "introsort_param cparam xs l h \<equiv> doN {
-    ASSERT(l\<le>h);
-    if h-l>1 then doN {
-      xs \<leftarrow> introsort_aux_param cparam xs l h (Discrete.log (h-l)*2);
-      xs \<leftarrow> final_insertion_sort_param cparam xs l h;
-      RETURN xs
-    } else RETURN xs
-  }"  
-
-  lemma introsort_param_refine: 
-    "\<lbrakk> (xs',xs)\<in>cdom_list_rel cparam; (l',l)\<in>Id; (h',h)\<in>Id
-    \<rbrakk> \<Longrightarrow> introsort_param cparam xs' l' h' \<le> \<Down>(cdom_list_rel cparam) (WO.introsort4 cparam xs l h)"
-    unfolding introsort_param_def WO.introsort4_def
-    apply (refine_rcg)
-    by auto
-
-      
-  lemma introsort_param_correct: 
-    assumes "(xs',xs)\<in>Id" "(l',l)\<in>Id" "(h',h)\<in>Id"
-    shows "introsort_param cparam xs' l' h' \<le> pslice_sort_spec cdom pless cparam xs l h"
-  proof -
-    note introsort_param_refine
-    also note WO.introsort4_correct
-    also note slice_sort_spec_xfer
-    finally show ?thesis 
-      unfolding pslice_sort_spec_def
-      apply refine_vcg
-      using assms unfolding cdom_list_rel_alt
-      by (simp add: in_br_conv)
-    
-  qed
-  
-  lemma introsort_param_correct': 
-    shows "(PR_CONST introsort_param, PR_CONST (pslice_sort_spec cdom pless)) \<in> Id \<rightarrow> Id \<rightarrow> Id \<rightarrow> Id \<rightarrow> \<langle>Id\<rangle>nres_rel"
-    using introsort_param_correct 
-    apply (intro fun_relI nres_relI) 
-    by simp
-  
-    
-    
-    
-end
-
-context parameterized_sort_impl_context begin
-
-
-sepref_register introsort_aux_param
-sepref_def introsort_aux_param_impl is "uncurry4 (PR_CONST introsort_aux_param)" 
-  :: "cparam_assn\<^sup>k *\<^sub>a (arr_assn)\<^sup>d *\<^sub>a size_assn\<^sup>k *\<^sub>a size_assn\<^sup>k *\<^sub>a size_assn\<^sup>k \<rightarrow>\<^sub>a arr_assn"
-  unfolding introsort_aux_param_def PR_CONST_def
-  apply (annot_snat_const "TYPE(size_t)")
-  by sepref
-  
-  
-sepref_register introsort_param
-sepref_def introsort_param_impl is "uncurry3 (PR_CONST introsort_param)" :: "cparam_assn\<^sup>k *\<^sub>a (arr_assn)\<^sup>d *\<^sub>a size_assn\<^sup>k *\<^sub>a size_assn\<^sup>k \<rightarrow>\<^sub>a arr_assn"
-  unfolding introsort_param_def PR_CONST_def
-  apply (annot_snat_const "TYPE(size_t)")
-  supply [intro!] = introsort_depth_limit_in_bounds_aux 
-  by sepref
-
-
-lemma introsort_param_impl_correct: "(uncurry3 introsort_param_impl, uncurry3 (PR_CONST (pslice_sort_spec cdom pless)))
-        \<in> cparam_assn\<^sup>k *\<^sub>a arr_assn\<^sup>d *\<^sub>a snat_assn\<^sup>k *\<^sub>a snat_assn\<^sup>k \<rightarrow>\<^sub>a arr_assn"
-  using introsort_param_impl.refine[FCOMP introsort_param_correct'] .
-  
-end
-*)
-
 
 
 end
