thys/examples/sorting/Sorting_Unguarded_Insertion_Sort.thy
@@ -1,10 +1,64 @@
+section \<open>Unguarded Insertion Sort\<close>
 theory Sorting_Unguarded_Insertion_Sort
 imports Sorting_Setup Sorting_Partially_Sorted
 begin
 
 
-(* TODO: Move *)
+  
+  (* TODO: Move, better name *)                     
+  lemma timerefine_R_cf_mono:
+    fixes R :: "_ \<Rightarrow> (_, enat) acost"
+    assumes "wfR'' R'"
+    shows "R\<le>R' \<Longrightarrow> \<Down> S (timerefine R c) \<le> \<Down> S (timerefine R' c)"
+    by (simp add: assms nrest_Rel_mono timerefine_R_mono_wfR'')
 
+lemma timerefine_mono_both: 
+  fixes R :: "_ \<Rightarrow> ('c, 'd::{complete_lattice,nonneg,mult_zero,ordered_semiring}) acost"
+  assumes "wfR'' R'"
+    and "R\<le>R'"
+  shows "c\<le>c' \<Longrightarrow> timerefine R c \<le> timerefine R' c'"
+  apply(cases c) apply simp
+  apply(cases c') apply (auto simp: less_eq_acost_def timerefine_def split: nrest.splits option.splits simp: le_fun_def)
+  subgoal  by (metis le_some_optE) 
+  proof (goal_cases)
+    case (1 x2 x2a x x2b x2c xa)
+    then have l: "\<And>ac. the_acost x2b ac \<le>  the_acost x2c ac"
+      apply(cases x2b; cases x2c) unfolding less_eq_acost_def  
+      apply auto
+      by (metis acost.sel less_eq_acost_def less_eq_option_Some)
+    show ?case
+      apply(rule Sum_any_mono)
+      subgoal using l apply(rule ordered_semiring_class.mult_mono)
+        subgoal using assms(2) unfolding le_fun_def
+          by (simp add: the_acost_mono)
+        subgoal by (simp add: needname_nonneg)
+        subgoal
+          by (simp add: needname_nonneg)
+        done
+      apply(rule wfR_finite_mult_left2) by fact
+  qed 
+
+
+lemma fun_upd_parallel_I: "f\<le>f' \<Longrightarrow> y\<le>y' \<Longrightarrow> f(x:=y) \<le> f'(x:=y')"
+  unfolding fun_upd_def le_fun_def  
+  by auto
+
+(* TODO: Move *)
+lemma timerefine_mono3: 
+  fixes R :: "_ \<Rightarrow> ('a, enat) acost"
+  assumes "wfR'' R"
+  shows "c\<le>c' \<Longrightarrow> R=R' \<Longrightarrow> timerefine R c \<le> timerefine R' c'"
+  apply simp
+  apply(rule timerefine_mono2)
+  using assms by auto
+
+
+    (* TODO: Move. DUP! *)
+    lemma if_rule: "(c \<Longrightarrow> x \<le> a) \<Longrightarrow> (~c \<Longrightarrow> x \<le> b) \<Longrightarrow> x \<le> (if c then a else b)"
+      by auto        
+
+
+subsection \<open>Auxiliary lemmas for option arrays\<close>
 
 text \<open>the time bound T needs to be agnostic of the length of the array.\<close>
 lemma mop_eo_extract_slice_refine: 
@@ -43,6 +97,8 @@ end
 
 
 
+subsection \<open>is_insert_unguarded\<close>
+
   context weak_ordering begin
 
   
@@ -67,20 +123,28 @@ end
         apply clarsimp
         unfolding is_insert_spec_aux_def
         apply (clarsimp;safe)
-        apply (smt greaterThanAtMost_iff less_trans linorder_neqE_nat nat_Suc_less_le_imp nat_le_Suc_less_imp nz_le_conv_less unfold_lt_to_le zero_order(3))
-        by (smt One_nat_def add_diff_cancel_left' atLeast0LessThan greaterThanAtMost_iff itrans le_less lessThan_iff less_Suc_eq_0_disj less_trans linorder_neqE_nat not_less_eq plus_1_eq_Suc unfold_lt_to_le wo_leI)
+         apply (smt greaterThanAtMost_iff less_trans linorder_neqE_nat nat_Suc_less_le_imp
+                      nat_le_Suc_less_imp nz_le_conv_less unfold_lt_to_le zero_order(3))
+        by (smt One_nat_def add_diff_cancel_left' atLeast0LessThan greaterThanAtMost_iff itrans
+                    le_less lessThan_iff less_Suc_eq_0_disj less_trans linorder_neqE_nat
+                    not_less_eq plus_1_eq_Suc unfold_lt_to_le wo_leI)
       subgoal
         using is_insert_spec_aux_def by blast
       done    
     
     (* TODO: Add type constraint to definition *)  
     abbreviation monadic_WHILEIET :: 
-      "('b \<Rightarrow> bool) \<Rightarrow> ('b \<Rightarrow> (char list, nat) acost) \<Rightarrow> ('b \<Rightarrow> (bool, (char list, enat) acost) nrest) \<Rightarrow> ('b \<Rightarrow> ('b, (char list, enat) acost) nrest) \<Rightarrow> 'b \<Rightarrow> ('b, (char list, enat) acost) nrest"
+      "('b \<Rightarrow> bool) \<Rightarrow> ('b \<Rightarrow> (char list, nat) acost) \<Rightarrow>
+       ('b \<Rightarrow> (bool, (char list, enat) acost) nrest) \<Rightarrow>
+       ('b \<Rightarrow> ('b, (char list, enat) acost) nrest) \<Rightarrow> 'b \<Rightarrow> ('b, (char list, enat) acost) nrest"
       where "monadic_WHILEIET I E b f s \<equiv> NREST.monadic_WHILEIET I E b f s"
       
-    definition "cost_is_insert_step :: (char list, nat) acost \<equiv> cost ''list_set'' 1 + (cost ''list_get'' 1 + (cost ''call'' 1 + (cost ''mop_cmp_v_idx'' 1 + cost ''sub'' 1 + cost ''if'' 1) + cost ''sub'' 1))"  
+  definition "cost_is_insert_step :: (char list, nat) acost \<equiv> cost ''list_set'' 1
+          + (cost ''list_get'' 1 + (cost ''call'' 1 
+          + (cost ''mop_cmp_v_idx'' 1 + cost ''sub'' 1 + cost ''if'' 1) + cost ''sub'' 1))"  
       
-    definition is_insert_unguarded :: "nat \<Rightarrow> 'a list \<Rightarrow> nat \<Rightarrow> ('a list,_) nrest" where "is_insert_unguarded N xs i \<equiv> doN {
+  definition is_insert_unguarded :: "nat \<Rightarrow> 'a list \<Rightarrow> nat \<Rightarrow> ('a list,_) nrest" where
+  "is_insert_unguarded N xs i \<equiv> doN {
       \<^cancel>\<open>(*ASSERT (\<exists>guard_idx. guard_idx<i \<and> \<not>xs!i\<^bold><xs!guard_idx);*)\<close>
       ASSERT (i<length xs);
       x \<leftarrow> mop_list_getN xs i;
@@ -117,162 +181,115 @@ end
       SPEC (is_insert_spec_aux xs i) (\<lambda>_. cost ''is_insert'' 1)
     }"  
     
-    (* TODO: Move. DUP! *)
-    lemma if_rule: "(c \<Longrightarrow> x \<le> a) \<Longrightarrow> (~c \<Longrightarrow> x \<le> b) \<Longrightarrow> x \<le> (if c then a else b)"
-      by auto        
-
   lemma lift_acost_propagate_minus: "lift_acost (t-t') = lift_acost t - lift_acost t' "
     unfolding lift_acost_def by (cases t; cases t'; auto)
       
   (* TODO: N \<rightarrow> N-1 ?*)  
   definition "cost_insert N \<equiv> 
     (lift_acost (N *m cost_is_insert_step) +
-      cost ''list_set'' 1 + (cost ''mop_cmp_v_idx'' 1 + cost ''sub'' 1 + cost ''if'' 1 + (cost ''list_get'' 1 + cost ''call'' 1)))"
+      cost ''list_set'' 1 + (cost ''mop_cmp_v_idx'' 1 + cost ''sub'' 1 + cost ''if'' 1
+       + (cost ''list_get'' 1 + cost ''call'' 1)))"
     
       
     definition "cost_is_insert_guarded_step :: (char list, nat) acost \<equiv>
-      cost ''list_set'' 1 + (cost ''list_get'' 1 + (cost ''call'' 1 + (cost ''mop_cmp_v_idx'' 1 + (cost ''if'' 1 + (0 + cost ''icmp_eq'' 1) + cost ''sub'' 1) + cost ''if'' 1) + cost ''sub'' 1))"
+      cost ''list_set'' 1 + (cost ''list_get'' 1 + (cost ''call'' 1 + (cost ''mop_cmp_v_idx'' 1 
+  + (cost ''if'' 1 + (0 + cost ''icmp_eq'' 1) + cost ''sub'' 1) + cost ''if'' 1) + cost ''sub'' 1))"
     
     definition "cost_insert_guarded N \<equiv> 
       lift_acost (N *m cost_is_insert_guarded_step) +
-        cost ''list_set'' 1 + cost ''mop_cmp_v_idx'' 1 + cost ''sub'' 1 + cost ''if'' 1 + cost ''list_get'' 1 + cost ''call'' 1
-        + cost ''if'' 1 + cost ''icmp_eq'' 1 + cost ''if'' 1 + cost ''list_get'' 1 + cost ''call'' 1"
+        cost ''list_set'' 1 + cost ''mop_cmp_v_idx'' 1 + cost ''sub'' 1 + cost ''if'' 1
+         + cost ''list_get'' 1 + cost ''call'' 1 + cost ''if'' 1 + cost ''icmp_eq'' 1 
+         + cost ''if'' 1 + cost ''list_get'' 1 + cost ''call'' 1"
     
 
-lemma finite_sum_gtzero_nat_cost:
-  "finite {a. the_acost (cost n m) a > (0::nat)}"
-  unfolding cost_def by (auto simp: zero_acost_def)
+  lemma finite_sum_gtzero_nat_cost:
+    "finite {a. the_acost (cost n m) a > (0::nat)}"
+    unfolding cost_def by (auto simp: zero_acost_def)
 
-    lemma is_insert_unguarded_correct: "is_insert_unguarded N xs i \<le> \<Down>Id (timerefine (TId (''is_insert'' := cost_insert N,   ''is_insert_g'' := cost_insert_guarded N)) (is_insert_spec_unguarded N xs i))"
-      unfolding is_insert_unguarded_def is_insert_spec_unguarded_def
-      apply (rule refine0)
-      apply (simp add: SPEC_timerefine_conv)
-      thm timerefine_SPECT
-      unfolding SPEC_def
-      unfolding SPECc2_def
-      unfolding has_stopper_def
-      apply(rule gwp_specifies_I)
-      apply (refine_vcg \<open>simp\<close> rules: gwp_monadic_WHILEIET if_rule)
+
+subsubsection \<open>Correctness Lemma\<close>
+
+abbreviation "E_ii N\<equiv>TId(''is_insert'' := cost_insert N,''is_insert_g'' := cost_insert_guarded N)"
+
+lemma is_insert_unguarded_correct: "is_insert_unguarded N xs i
+   \<le> \<Down>Id (timerefine (E_ii N) (is_insert_spec_unguarded N xs i))"
+    unfolding is_insert_unguarded_def is_insert_spec_unguarded_def
+    apply (rule refine0)
+    apply (simp add: SPEC_timerefine_conv)
+    thm timerefine_SPECT
+    unfolding SPEC_def
+    unfolding SPECc2_def
+    unfolding has_stopper_def
+    apply(rule gwp_specifies_I)
+    apply (refine_vcg \<open>simp\<close> rules: gwp_monadic_WHILEIET if_rule)
+    subgoal
+      apply(auto simp:  wfR2_def the_acost_zero_app) 
+      unfolding cost_is_insert_step_def
+      apply(auto simp: norm_cost ) 
+      by(auto simp: finite_sum_gtzero_nat_cost)
+    subgoal for s a b
+      apply (rule loop_body_conditionI)
       subgoal
-        apply(auto simp:  wfR2_def the_acost_zero_app) 
         unfolding cost_is_insert_step_def
-        apply(auto simp: norm_cost ) 
-        by(auto simp: finite_sum_gtzero_nat_cost)
-      subgoal for s a b
-        apply (rule loop_body_conditionI)
-        subgoal
-          unfolding cost_is_insert_step_def
-          apply(simp add: norm_cost)
-          apply sc_solve by auto 
-        subgoal 
-          apply (clarsimp simp: cost_is_insert_step_def norm_cost)
-          apply sc_solve
-          apply (simp add: one_enat_def algebra_simps)
-          apply (intro conjI)
-          apply (metis Suc_diff_Suc diff_diff_cancel diff_le_self diff_zero le_diff_conv le_trans nat_add_left_cancel_le neq0_conv zero_less_diff)
-          subgoal 
-            apply (subgoal_tac "1 + (N+b-Suc i) = N+b-i")
-            apply simp 
-            apply (simp)
-            apply (metis Suc_diff_Suc diff_diff_cancel diff_le_self diff_zero le_diff_conv le_trans nat_add_left_cancel_le neq0_conv zero_less_diff)
-            done
-          subgoal 
-            by (metis Suc_diff_Suc Suc_pred add_diff_cancel_left' le_diff_conv le_eq_less_or_eq le_simps(3) linorder_not_le)
-          done
-        subgoal
-          apply simp  
-          apply (intro conjI)
-          subgoal by (metis (full_types) diff_is_0_eq' not_less zero_le)
-          subgoal by (metis Suc_le_eq Suc_pred le_diff_conv le_eq_less_or_eq nat_add_left_cancel_le)
-          subgoal by linarith
-          subgoal by (metis atLeastAtMost_iff diff_Suc_less diff_le_self le_trans linorder_not_le nth_list_update')
-          subgoal by (smt Suc_diff_Suc diff_zero greaterThanAtMost_iff le_eq_less_or_eq le_less_trans le_simps(3) nth_list_update_eq nth_list_update_neq)
-        done
-      done  
-      subgoal for _ _ i'
-        apply (rule loop_exit_conditionI)
-        apply (refine_vcg \<open>simp\<close>)
-        apply simp
+        apply(simp add: norm_cost)
+        apply sc_solve by auto 
+      subgoal 
+        apply (clarsimp simp: cost_is_insert_step_def norm_cost)
+        apply sc_solve
+        apply (simp add: one_enat_def algebra_simps)
         apply (intro conjI)
-        subgoal
-          unfolding is_insert_spec_aux_def
-          apply (rule exI[where x=i']) 
-          by auto
-        subgoal
-          apply (simp add: algebra_simps lift_acost_diff_to_the_right)
-          apply (simp add: cost_insert_def)
-          apply (clarsimp simp: cost_is_insert_step_def costmult_add_distrib costmult_cost lift_acost_propagate lift_acost_cost timerefineA_update_apply_same_cost')
-          apply sc_solve
-          by auto
+        apply (metis Suc_diff_Suc diff_diff_cancel diff_le_self diff_zero le_diff_conv le_trans
+                    nat_add_left_cancel_le neq0_conv zero_less_diff)
+        subgoal 
+          apply (subgoal_tac "1 + (N+b-Suc i) = N+b-i")
+          apply simp 
+          apply (simp)
+          apply (metis Suc_diff_Suc diff_diff_cancel diff_le_self diff_zero le_diff_conv
+                      le_trans nat_add_left_cancel_le neq0_conv zero_less_diff)
+          done
+        subgoal 
+          by (metis Suc_diff_Suc Suc_pred add_diff_cancel_left' le_diff_conv le_eq_less_or_eq
+                    le_simps(3) linorder_not_le)
         done
-          
-      subgoal by auto
-      subgoal by auto
+      subgoal
+        apply simp  
+        apply (intro conjI)
+        subgoal by (metis (full_types) diff_is_0_eq' not_less zero_le)
+        subgoal by (metis Suc_le_eq Suc_pred le_diff_conv le_eq_less_or_eq nat_add_left_cancel_le)
+        subgoal by linarith
+        subgoal by (metis atLeastAtMost_iff diff_Suc_less diff_le_self le_trans
+                          linorder_not_le nth_list_update')
+        subgoal by (smt Suc_diff_Suc diff_zero greaterThanAtMost_iff le_eq_less_or_eq le_less_trans
+                          le_simps(3) nth_list_update_eq nth_list_update_neq)
       done
-    
-    
-    (*    
-        
-    definition "is_insert_spec N GUARDED xs i \<equiv> doN {
-      ASSERT (i<length xs \<and> (\<not>GUARDED \<longrightarrow> 0<i \<and> \<not>xs!i\<^bold><xs!0));
-      SPEC (is_insert_spec_aux xs i) (\<lambda>_. N)
-    }"  
-
-    text \<open>When unguarded, the first element of the list cannot change\<close>
-    lemma is_insert_spec_alt: "is_insert_spec GUARDED xs i = doN {
-      ASSERT (i<length xs \<and> (\<not>GUARDED \<longrightarrow> 0<i \<and> \<not>xs!i\<^bold><xs!0));
-      SPEC (\<lambda>xs'. is_insert_spec_aux xs i xs' \<and> (\<not>GUARDED \<longrightarrow> xs'!0 = xs!0))
-    }"
-      unfolding is_insert_spec_def 
-      apply (simp only: pw_eq_iff refine_pw_simps; clarsimp; safe)
-      unfolding is_insert_spec_aux_def
-      apply clarsimp
-      by (metis Suc_leI Suc_to_right atLeast0LessThan greaterThanAtMost_iff lessThan_iff not_less_eq)
-    
-    lemma is_insert_correct: "is_insert GUARDED xs i \<le> is_insert_spec GUARDED xs i"
-      unfolding is_insert_def is_insert_spec_def
-      apply (refine_vcg WHILEIT_rule[where R="measure snd"])
-      apply clarsimp_all
-      subgoal by (metis Suc_lessI Suc_to_right)
-      subgoal by linarith
-      subgoal by (metis Suc_lessI Suc_pred greaterThanAtMost_iff le_less_trans nth_list_update')
-    
-      subgoal for xs' i'
+    done  
+    subgoal for _ _ i'
+      apply (rule loop_exit_conditionI)
+      apply (refine_vcg \<open>simp\<close>)
+      apply simp
+      apply (intro conjI)
+      subgoal
         unfolding is_insert_spec_aux_def
         apply (rule exI[where x=i']) 
         by auto
-        
+      subgoal
+        apply (simp add: algebra_simps lift_acost_diff_to_the_right)
+        apply (simp add: cost_insert_def)
+        apply (clarsimp simp: cost_is_insert_step_def costmult_add_distrib costmult_cost
+                        lift_acost_propagate lift_acost_cost timerefineA_update_apply_same_cost')
+        apply sc_solve
+        by auto
       done
-      
-    definition is_insert2 :: "bool \<Rightarrow> 'a list \<Rightarrow> nat \<Rightarrow> 'a list nres" where "is_insert2 GUARDED xs i \<equiv> doN {
-      ASSERT ((\<not>GUARDED\<longrightarrow>0<i) \<and> i<length xs);
-      
-      xs \<leftarrow> mop_to_eo_conv xs;
-      
-      (x,xs) \<leftarrow> mop_eo_extract xs i;
+        
+    subgoal by auto
+    subgoal by auto
+    done
     
-      (xs,i)\<leftarrow>monadic_WHILEIT (\<lambda>(xs',i'). True) 
-        (\<lambda>(xs,i). if \<not>GUARDED \<or> i>0 then doN { ASSERT (i>0); mop_cmpo_v_idx xs x (i-1)} else RETURN False) (\<lambda>(xs,i). doN {
-          ASSERT (i>0);
-          (t,xs) \<leftarrow> mop_eo_extract xs (i-1);
-          xs \<leftarrow> mop_eo_set xs i t;
-          let i = i-1;
-          RETURN (xs,i)
-        }) (xs,i);
     
-      xs \<leftarrow> mop_eo_set xs i x;  
-      
-      xs \<leftarrow> mop_to_wo_conv xs;
-      
-      RETURN xs
-    }"
-    *)
-    
-    (*abbreviation "mop_eo_extract' \<equiv> mop_eo_extract (\<lambda>_. lift_acost mop_array_nth_cost)"
-    abbreviation "mop_eo_set' \<equiv> mop_eo_set (\<lambda>_. lift_acost mop_array_upd_cost)"
-    *)
-    
-    definition is_insert2_unguarded :: "nat \<Rightarrow> 'a list \<Rightarrow> nat \<Rightarrow> ('a list,_) nrest" where "is_insert2_unguarded N xs i \<equiv> doN {
+subsection \<open>is_insert_unguarded2\<close>
+
+  definition is_insert_unguarded2 :: "nat \<Rightarrow> 'a list \<Rightarrow> nat \<Rightarrow> ('a list,_) nrest" where
+  "is_insert_unguarded2 N xs i \<equiv> doN {
       \<^cancel>\<open>(*ASSERT (\<exists>guard_idx. guard_idx<i \<and> \<not>xs!i\<^bold><xs!guard_idx);*)\<close>
       ASSERT (i<length xs);
       
@@ -301,16 +318,20 @@ lemma finite_sum_gtzero_nat_cost:
 
     
     
-    definition "ii2_loop_rel \<equiv> {((xs',i'), (xs,i)). i'=i \<and> length xs' = length xs \<and> i<length xs \<and> (\<forall>j\<in>{0..<length xs}-{i}. xs'!j = Some (xs!j)) \<and> xs'!i=None}"
+  definition "ii2_loop_rel \<equiv> {((xs',i'), (xs,i)). i'=i \<and> length xs' = length xs \<and> i<length xs
+       \<and> (\<forall>j\<in>{0..<length xs}-{i}. xs'!j = Some (xs!j)) \<and> xs'!i=None}"
     
-    abbreviation "TR_ii2 \<equiv> TId(
+    abbreviation "E_iiu2_aux \<equiv> TId(
       ''list_get'' := lift_acost mop_array_nth_cost,
       ''list_set'' := lift_acost mop_array_upd_cost,
       ''mop_cmp_v_idx'' := cost ''cmpo_v_idx'' 1
     )"
     
-    lemma is_insert2_unguarded_refine: "is_insert2_unguarded N xs i \<le>\<Down>(\<langle>Id\<rangle>list_rel) (timerefine TR_ii2 (is_insert_unguarded N xs i))"
-      unfolding is_insert2_unguarded_def is_insert_unguarded_def
+subsubsection \<open>Refinement Lemma\<close>
+
+  lemma is_insert_unguarded2_refine: "is_insert_unguarded2 N xs i
+     \<le> \<Down>(\<langle>Id\<rangle>list_rel) (timerefine E_iiu2_aux (is_insert_unguarded N xs i))"
+      unfolding is_insert_unguarded2_def is_insert_unguarded_def
       supply [simp del] = conc_Id
       
       unfolding mop_oarray_extract_def mop_oarray_upd_def
@@ -378,15 +399,18 @@ lemma finite_sum_gtzero_nat_cost:
         subgoal by (auto simp: in_set_conv_nth nth_list_update intro: list_eq_iff_nth_eq[THEN iffD2])
         subgoal by force
         subgoal by simp
-        subgoal by (auto simp add: timerefineA_propagate timerefineA_update_apply_same_cost' lift_acost_zero)
-        subgoal by (auto simp: ii2_loop_rel_def nth_list_update in_set_conv_nth intro: list_eq_iff_nth_eq[THEN iffD2])
+        subgoal by (auto simp add: timerefineA_propagate timerefineA_update_apply_same_cost'
+                          lift_acost_zero)
+        subgoal by (auto simp: ii2_loop_rel_def nth_list_update in_set_conv_nth
+                        intro: list_eq_iff_nth_eq[THEN iffD2])
         done
       done
       
-      
-    lemma is_insert3_unguarded_refine': "\<lbrakk> (xs,xs')\<in>slicep_rel l h; (i,i')\<in>idx_shift_rel l; i<h \<rbrakk> 
-      \<Longrightarrow> is_insert2_unguarded N xs i \<le>\<Down>(slice_rel xs l h) (timerefine TId (is_insert2_unguarded N xs' i'))"
-      unfolding is_insert2_unguarded_def 
+subsubsection \<open>Refinement Lemma -- slice_rel\<close>
+
+    lemma is_insert_unguarded3_refine': "\<lbrakk> (xs,xs')\<in>slicep_rel l h; (i,i')\<in>idx_shift_rel l; i<h \<rbrakk> 
+      \<Longrightarrow> is_insert_unguarded2 N xs i \<le>\<Down>(slice_rel xs l h) (timerefine TId (is_insert_unguarded2 N xs' i'))"
+      unfolding is_insert_unguarded2_def 
       unfolding mop_oarray_extract_def mop_oarray_upd_def
       
       supply [simp del] = conc_Id
@@ -404,11 +428,16 @@ lemma finite_sum_gtzero_nat_cost:
       )
       supply [[goals_limit=20]]
       apply refine_dref_type
-      apply (all \<open>(assumption|simp (no_asm);fail|simp add: idx_shift_rel_def;simp add: slice_map slice_rel_def slicep_rel_def in_br_conv)?\<close>)
+      apply (all \<open>(assumption|simp (no_asm);fail|simp add: idx_shift_rel_def;
+                    simp add: slice_map slice_rel_def slicep_rel_def in_br_conv)?\<close>)
       subgoal by linarith
       done
       
+  (* TODO: find a better format here *)
+  abbreviation "E_iiu2 N \<equiv> pp E_iiu2_aux (E_ii N)"
+
         
+subsubsection \<open>Sideconditions\<close>
 
     (* TODO: Move. Side-conditions? @Max *)   
     \<^cancel>\<open>
@@ -426,46 +455,46 @@ lemma finite_sum_gtzero_nat_cost:
       assumes WF2: "wfR'' TR\<^sub>2"
       shows "m\<^sub>1 \<le> \<Down>(R\<^sub>1 O R\<^sub>2) (timerefine (pp TR\<^sub>1 TR\<^sub>2) m\<^sub>3)"
       apply (rule order_trans[OF assms(1)])
-      apply (simp add: conc_fun_complete_lattice_chain[symmetric] timerefine_iter2[OF WF1 WF2, symmetric]) (* TODO: Why the special version conc_fun_chain for enat? *)
+      apply (simp add: conc_fun_complete_lattice_chain[symmetric] timerefine_iter2[OF WF1 WF2, symmetric])
+         (* TODO: Why the special version conc_fun_chain for enat? *)
       apply (rule nrest_Rel_mono)
       apply (subst timerefine_comm_concfun[symmetric])
       apply fact
       apply (rule timerefine_mono2[OF WF1])
       by fact\<close>
       
-        
-    find_theorems pp fun_upd
-    find_theorems timerefineA fun_upd  
       
-    abbreviation "TR_ii3 N \<equiv> pp TR_ii2 (TId(''is_insert'' := cost_insert N,  ''is_insert_g'' := cost_insert_guarded N))" (* @Max: what's a good format here? *)
-
     (* TODO: enable this! by fixing timerefine_comm_concfun *)
   \<^cancel>\<open>
-    lemma is_insert3_unguarded_correct'_right: 
-      assumes "(xs,xs')\<in>slicep_rel l h" "(i,i')\<in>idx_shift_rel l" "i<h"
-      shows "is_insert2_unguarded N xs i \<le>\<Down>(slice_rel xs l h) (timerefine (TR_ii3 N) (is_insert_spec_unguarded N xs' i'))"
-    proof -
-      note is_insert3_unguarded_refine'[OF assms]
-      also note is_insert2_unguarded_refine
-      also note is_insert_unguarded_correct
-      finally show ?thesis
-        apply (simp add: pp_TId_absorbs_left pp_TId_absorbs_right)
-        apply rprems
-        apply force+
-        done
-    qed
+  lemma is_insert3_unguarded_correct'_right: 
+    assumes "(xs,xs')\<in>slicep_rel l h" "(i,i')\<in>idx_shift_rel l" "i<h"
+    shows "is_insert_unguarded2 N xs i
+       \<le>\<Down>(slice_rel xs l h) (timerefine (TR_ii3 N) (is_insert_spec_unguarded N xs' i'))"
+  proof -
+    note is_insert3_unguarded_refine'[OF assms]
+    also note is_insert_unguarded2_refine
+    also note is_insert_unguarded_correct
+    finally show ?thesis
+      apply (simp add: pp_TId_absorbs_left pp_TId_absorbs_right)
+      apply rprems
+      apply force+
+      done
+  qed
 \<close>
+        
+subsubsection \<open>Correctness lemma\<close>
 
   
-    lemma is_insert3_unguarded_correct': 
+    lemma is_insert_unguarded2_correct': 
       assumes "(xs,xs')\<in>slicep_rel l h" "(i,i')\<in>idx_shift_rel l" "i<h"
-      shows "is_insert2_unguarded N xs i \<le>\<Down>(slice_rel xs l h) (timerefine (TR_ii3 N) (is_insert_spec_unguarded N xs' i'))"
+      shows "is_insert_unguarded2 N xs i
+         \<le> \<Down>(slice_rel xs l h) (timerefine (E_iiu2 N) (is_insert_spec_unguarded N xs' i'))"
       apply(rule order.trans)
-      apply(rule is_insert3_unguarded_refine'[OF assms])
+      apply(rule is_insert_unguarded3_refine'[OF assms])
       apply(rule nrest_Rel_mono)
       apply (simp add: timerefine_id)
       apply(rule order.trans)
-       apply(rule is_insert2_unguarded_refine)
+       apply(rule is_insert_unguarded2_refine)
       apply simp
       apply(subst timerefine_iter2[symmetric])
       subgoal by(auto intro!: wfR''_upd)
@@ -476,8 +505,10 @@ lemma finite_sum_gtzero_nat_cost:
        apply(rule is_insert_unguarded_correct)
       by simp 
         
+subsection \<open>is_insert_guarded\<close>
 
-    definition is_insert_guarded :: "'a list \<Rightarrow> nat \<Rightarrow> ('a list,_) nrest" where "is_insert_guarded xs i \<equiv> doN {
+  definition is_insert_guarded :: "'a list \<Rightarrow> nat \<Rightarrow> ('a list,_) nrest" where
+    "is_insert_guarded xs i \<equiv> doN {
       \<^cancel>\<open>(*ASSERT (\<exists>guard_idx. guard_idx<i \<and> \<not>xs!i\<^bold><xs!guard_idx);*)\<close>
       ASSERT (i<length xs);
       x \<leftarrow> mop_list_getN xs i;
@@ -517,8 +548,13 @@ lemma finite_sum_gtzero_nat_cost:
     }"  
     
     
-    
-    lemma is_insert_guarded_correct: "is_insert_guarded xs i \<le> \<Down>Id (timerefine (TId (''is_insert'' := cost_insert N, ''is_insert_g'' := cost_insert_guarded i)) (is_insert_spec_guarded xs i))"
+subsubsection \<open>Correctness Lemma\<close>
+
+  abbreviation "E_iig N i \<equiv> TId (''is_insert'' := cost_insert N,
+                               ''is_insert_g'' := cost_insert_guarded i)"
+
+  lemma is_insert_guarded_correct: "is_insert_guarded xs i
+     \<le> \<Down>Id (timerefine (E_iig N i) (is_insert_spec_guarded xs i))"
       unfolding is_insert_guarded_def is_insert_spec_guarded_def
       apply (rule refine0)
       apply (simp add: SPEC_timerefine_conv)
@@ -541,8 +577,8 @@ lemma finite_sum_gtzero_nat_cost:
           apply (fastforce simp: is_insert_spec_aux_def)
           
           apply (clarsimp simp: 
-            cost_is_insert_guarded_step_def costmult_add_distrib costmult_cost lift_acost_propagate lift_acost_cost algebra_simps cost_zero
-            cost_insert_guarded_def timerefineA_cost
+            cost_is_insert_guarded_step_def costmult_add_distrib costmult_cost lift_acost_propagate
+            lift_acost_cost algebra_simps cost_zero cost_insert_guarded_def timerefineA_cost
             )
         
           apply sc_solve
@@ -558,7 +594,8 @@ lemma finite_sum_gtzero_nat_cost:
           apply(simp add: norm_cost)
           apply sc_solve by auto 
         subgoal 
-          apply (clarsimp simp: cost_is_insert_guarded_step_def costmult_add_distrib costmult_cost lift_acost_propagate lift_acost_cost)
+          apply (clarsimp simp: cost_is_insert_guarded_step_def costmult_add_distrib costmult_cost 
+                                lift_acost_propagate lift_acost_cost)
           apply sc_solve
           apply (simp add: one_enat_def algebra_simps)
           done
@@ -567,7 +604,8 @@ lemma finite_sum_gtzero_nat_cost:
           apply (intro conjI)
           apply linarith
           apply clarsimp
-          by (metis Suc_lessI Suc_pred greaterThanAtMost_iff le_less_trans nth_list_update_eq nth_list_update_neq)
+          by (metis Suc_lessI Suc_pred greaterThanAtMost_iff le_less_trans nth_list_update_eq
+                    nth_list_update_neq)
       done  
       subgoal for _ _ i'
         apply (rule loop_exit_conditionI)
@@ -581,7 +619,8 @@ lemma finite_sum_gtzero_nat_cost:
         subgoal
           apply (simp add: algebra_simps lift_acost_diff_to_the_right)
           apply (simp add: cost_insert_guarded_def)
-          apply (clarsimp simp: cost_is_insert_guarded_step_def costmult_add_distrib costmult_cost lift_acost_propagate lift_acost_cost timerefineA_update_apply_same_cost')
+          apply (clarsimp simp: cost_is_insert_guarded_step_def costmult_add_distrib costmult_cost
+                        lift_acost_propagate lift_acost_cost timerefineA_update_apply_same_cost')
           apply sc_solve
           apply (auto simp flip: plus_enat_simps simp: algebra_simps)
           done
@@ -589,8 +628,12 @@ lemma finite_sum_gtzero_nat_cost:
           
       subgoal by auto
       done
+
+
+subsection \<open>is_insert_guarded2\<close>
     
-    definition is_insert2_guarded :: "'a list \<Rightarrow> nat \<Rightarrow> ('a list,_) nrest" where "is_insert2_guarded xs i \<equiv> doN {
+  definition is_insert_guarded2 :: "'a list \<Rightarrow> nat \<Rightarrow> ('a list,_) nrest" where
+    "is_insert_guarded2 xs i \<equiv> doN {
       \<^cancel>\<open>(*ASSERT (\<exists>guard_idx. guard_idx<i \<and> \<not>xs!i\<^bold><xs!guard_idx);*)\<close>
       ASSERT (i<length xs);
       
@@ -621,9 +664,11 @@ lemma finite_sum_gtzero_nat_cost:
       RETURN xs
     }"
     
+subsubsection \<open>Refinement lemma\<close>
     
-    lemma is_insert2_guarded_refine: "is_insert2_guarded xs i \<le>\<Down>(\<langle>Id\<rangle>list_rel) (timerefine TR_ii2 (is_insert_guarded xs i))"
-      unfolding is_insert2_guarded_def is_insert_guarded_def
+  lemma is_insert_guarded2_refine: "is_insert_guarded2 xs i
+    \<le> \<Down>(\<langle>Id\<rangle>list_rel) (timerefine E_iiu2_aux (is_insert_guarded xs i))"
+      unfolding is_insert_guarded2_def is_insert_guarded_def
       unfolding mop_oarray_upd_def mop_oarray_extract_def
       supply [simp del] = conc_Id
       
@@ -692,16 +737,21 @@ lemma finite_sum_gtzero_nat_cost:
         apply refine_dref_type
         unfolding ii2_loop_rel_def
         subgoal by auto
-        subgoal by (auto simp: in_set_conv_nth nth_list_update intro: list_eq_iff_nth_eq[THEN iffD2])
+        subgoal by (auto simp: in_set_conv_nth nth_list_update
+                        intro: list_eq_iff_nth_eq[THEN iffD2])
         subgoal by force
         subgoal by simp
-        subgoal by (auto simp add: timerefineA_propagate timerefineA_update_apply_same_cost' lift_acost_zero)
-        subgoal by (auto simp: ii2_loop_rel_def nth_list_update in_set_conv_nth intro: list_eq_iff_nth_eq[THEN iffD2])
+        subgoal by (auto simp add: timerefineA_propagate timerefineA_update_apply_same_cost'
+                          lift_acost_zero)
+        subgoal by (auto simp: ii2_loop_rel_def nth_list_update in_set_conv_nth 
+                      intro: list_eq_iff_nth_eq[THEN iffD2])
         done
       done
     
+subsection \<open>is_insert3_guarded\<close>
     
-    definition is_insert3_guarded :: "'a list \<Rightarrow> nat \<Rightarrow> nat \<Rightarrow> ('a list,_) nrest" where "is_insert3_guarded xs l i \<equiv> doN {
+  definition is_insert3_guarded :: "'a list \<Rightarrow> nat \<Rightarrow> nat \<Rightarrow> ('a list,_) nrest" where
+    "is_insert3_guarded xs l i \<equiv> doN {
       \<^cancel>\<open>(*ASSERT (\<exists>guard_idx. guard_idx<i \<and> \<not>xs!i\<^bold><xs!guard_idx);*)\<close>
       ASSERT (i<length xs);
       
@@ -734,8 +784,8 @@ lemma finite_sum_gtzero_nat_cost:
     
   
     lemma is_insert3_guarded_refine': "\<lbrakk> (xs,xs')\<in>slicep_rel l h; (i,i')\<in>idx_shift_rel l; i<h \<rbrakk> 
-      \<Longrightarrow> is_insert3_guarded xs l i \<le>\<Down>(slice_rel xs l h) (timerefine TId (is_insert2_guarded xs' i'))"
-      unfolding is_insert2_guarded_def is_insert3_guarded_def
+      \<Longrightarrow> is_insert3_guarded xs l i \<le>\<Down>(slice_rel xs l h) (timerefine TId (is_insert_guarded2 xs' i'))"
+      unfolding is_insert_guarded2_def is_insert3_guarded_def
       unfolding mop_oarray_upd_def mop_oarray_extract_def
       
       supply [simp del] = conc_Id
@@ -754,22 +804,24 @@ lemma finite_sum_gtzero_nat_cost:
       )
       supply [[goals_limit=20]]
       apply refine_dref_type
-      apply (all \<open>(assumption|simp (no_asm);fail|simp add: idx_shift_rel_def;simp add: slice_map slice_rel_def slicep_rel_def in_br_conv)?\<close>)
+      apply (all \<open>(assumption|simp (no_asm);fail|simp add: idx_shift_rel_def;
+        simp add: slice_map slice_rel_def slicep_rel_def in_br_conv)?\<close>)
       subgoal by linarith
       done
     
-    abbreviation "TR_ii3_guarded N \<equiv> pp TR_ii2 (TId(''is_insert'' := cost_insert N, ''is_insert_g'' := cost_insert_guarded N))" (* @Max: what's a good format here? *)
+  abbreviation "TR_ii3_guarded N \<equiv> pp E_iiu2_aux (E_ii N)"
       
     (* TODO: enable this! by fixing timerefine_comm_concfun *)
   \<^cancel>\<open>
     lemma is_insert3_guarded_correct'_right: 
       assumes "(xs,xs')\<in>slicep_rel l h" "(i,i')\<in>idx_shift_rel l" "i<h"
-      shows "is_insert3_guarded xs l i \<le>\<Down>(slice_rel xs l h) (timerefine (TR_ii3_guarded (i-l)) (is_insert_spec_guarded xs' i'))"
+      shows "is_insert3_guarded xs l i 
+        \<le>\<Down>(slice_rel xs l h) (timerefine (TR_ii3_guarded (i-l)) (is_insert_spec_guarded xs' i'))"
     proof -
       from assms(2) have [simp]: "i' = i-l" by (auto simp: idx_shift_rel_def)
     
       note is_insert3_guarded_refine'[OF assms]
-      also note is_insert2_guarded_refine
+      also note is_insert_guarded2_refine
       also note is_insert_guarded_correct
       finally show ?thesis
         apply (simp add: pp_TId_absorbs_left pp_TId_absorbs_right)
@@ -780,7 +832,8 @@ lemma finite_sum_gtzero_nat_cost:
 
     lemma is_insert3_guarded_correct': 
       assumes "(xs,xs')\<in>slicep_rel l h" "(i,i')\<in>idx_shift_rel l" "i<h"
-      shows "is_insert3_guarded xs l i \<le>\<Down>(slice_rel xs l h) (timerefine (TR_ii3_guarded (i-l)) (is_insert_spec_guarded xs' i'))"
+      shows "is_insert3_guarded xs l i 
+          \<le>\<Down>(slice_rel xs l h) (timerefine (TR_ii3_guarded (i-l)) (is_insert_spec_guarded xs' i'))"
     proof -
       from assms(2) have [simp]: "i' = i-l" by (auto simp: idx_shift_rel_def)
       show ?thesis
@@ -789,7 +842,7 @@ lemma finite_sum_gtzero_nat_cost:
       apply(rule nrest_Rel_mono)
       apply (simp add: timerefine_id)
       apply(rule order.trans)
-       apply(rule is_insert2_guarded_refine)
+       apply(rule is_insert_guarded2_refine)
       apply simp
       apply(subst timerefine_iter2[symmetric])
       subgoal by(auto intro!: wfR''_upd)
@@ -802,13 +855,14 @@ lemma finite_sum_gtzero_nat_cost:
   qed
         
 end
-  
-find_theorems mop_oarray_extract mop_eo_extract
+
+subsection \<open>is_insert_unguarded4\<close>
 
 context sort_impl_context begin
 
 
-    definition is_insert_unguarded4 :: "nat \<Rightarrow> 'a list \<Rightarrow> nat \<Rightarrow> ('a list,_) nrest" where "is_insert_unguarded4 N xs i \<equiv> doN {
+  definition is_insert_unguarded4 :: "nat \<Rightarrow> 'a list \<Rightarrow> nat \<Rightarrow> ('a list,_) nrest" where
+    "is_insert_unguarded4 N xs i \<equiv> doN {
       \<^cancel>\<open>(*ASSERT (\<exists>guard_idx. guard_idx<i \<and> \<not>xs!i\<^bold><xs!guard_idx);*)\<close>
       ASSERT (i<length xs);
       
@@ -839,13 +893,14 @@ context sort_impl_context begin
 
   lemma is_insert_unguarded4_refines:
     "(xs,xs')\<in>Id \<Longrightarrow> (i,i')\<in>Id \<Longrightarrow> 
-      is_insert_unguarded4 N xs i \<le> \<Down>Id (timerefine TR_cmp_swap (is_insert2_unguarded N xs' i'))"
+      is_insert_unguarded4 N xs i \<le> \<Down>Id (timerefine TR_cmp_swap (is_insert_unguarded2 N xs' i'))"
     supply conc_Id[simp del] mop_cmpo_v_idx_def[simp del]
-    unfolding is_insert_unguarded4_def is_insert2_unguarded_def
+    unfolding is_insert_unguarded4_def is_insert_unguarded2_def
     supply [refine] = mop_to_eo_conv_refine  mop_to_wo_conv_refines
           cmpo_v_idx2'_refines_mop_cmpo_v_idx_with_E
           mop_oarray_extract_refines mop_oarray_upd_refines
-    apply(refine_rcg MIf_refine SPECc2_refine' bindT_refine_conc_time_my_inres monadic_WHILEIT_refine' )
+    apply(refine_rcg MIf_refine SPECc2_refine' 
+            bindT_refine_conc_time_my_inres monadic_WHILEIT_refine' )
                         apply refine_dref_type
   apply(all \<open>(intro  preserves_curr_other_updI wfR''_upd wfR''_TId preserves_curr_TId)?\<close>)
   apply (simp_all (no_asm))
@@ -866,6 +921,7 @@ context sort_impl_context begin
     by sepref
     
 
+subsection \<open>is_insert_guarded4\<close>
   
 
   definition is_insert_guarded4 :: "'a list \<Rightarrow> nat \<Rightarrow> nat \<Rightarrow> ('a list,_) nrest"
@@ -909,7 +965,8 @@ context sort_impl_context begin
     supply [refine] = mop_to_eo_conv_refine  mop_to_wo_conv_refines
           cmpo_v_idx2'_refines_mop_cmpo_v_idx_with_E
           mop_oarray_extract_refines mop_oarray_upd_refines
-    apply(refine_rcg MIf_refine SPECc2_refine' bindT_refine_conc_time_my_inres monadic_WHILEIT_refine' )
+    apply(refine_rcg MIf_refine SPECc2_refine' bindT_refine_conc_time_my_inres
+          monadic_WHILEIT_refine' )
                         apply refine_dref_type
   apply(all \<open>(intro  preserves_curr_other_updI wfR''_upd wfR''_TId preserves_curr_TId)?\<close>)
   apply (simp_all (no_asm))
@@ -928,6 +985,7 @@ context sort_impl_context begin
 end    
 
 
+subsection \<open>Insertion sort - specification unguarded\<close>
 
 context weak_ordering begin
 
@@ -941,7 +999,8 @@ context weak_ordering begin
       apply (clarsimp simp: nth_append nth_Cons split: nat.splits)
       apply (safe; clarsimp?)
       subgoal for j k
-        by (metis One_nat_def Suc_le_eq add.commute add_Suc_right add_diff_cancel_left' add_diff_inverse_nat greaterThanAtMost_iff less_diff_conv plus_1_eq_Suc zero_less_Suc)
+        by (metis One_nat_def Suc_le_eq add.commute add_Suc_right add_diff_cancel_left'
+              add_diff_inverse_nat greaterThanAtMost_iff less_diff_conv plus_1_eq_Suc zero_less_Suc)
       subgoal by (metis add_Suc leI le_add_diff_inverse2)
       done
     done
@@ -1040,17 +1099,14 @@ context weak_ordering begin
           apply (intro impI)
           apply (subgoal_tac "ja < length xs")
           apply simp
-          apply (metis Suc_to_right asym greaterThanAtMost_iff itrans leI le_eq_less_or_eq less_Suc_eq_le)
+           apply (metis Suc_to_right asym greaterThanAtMost_iff itrans
+                      leI le_eq_less_or_eq less_Suc_eq_le)
           apply linarith
           done
         done
       done  
     done (* TODO: Understand this proof! *)
     
-    
-        
-    
-      
     
   definition "sort_one_more_spec_unguarded N xs i h \<equiv> doN {
       ASSERT (i<length xs \<and> sorted_wrt_lt (\<^bold><) (take i xs) \<and> h\<le>length xs);
@@ -1071,12 +1127,9 @@ context weak_ordering begin
   *)
   
   lemma is_insert_unguarded_sorts_one_more: 
-    "i<h \<Longrightarrow> is_insert_spec_unguarded N xs i \<le> \<Down>Id (timerefine TId (sort_one_more_spec_unguarded N xs i h))"
-  
+    "i<h \<Longrightarrow> is_insert_spec_unguarded N xs i \<le> \<Down>Id (timerefine TId (sort_one_more_spec_unguarded N xs i h))"  
     (*apply (intro fun_relI nrest_relI')    *)
-    
-    find_theorems TId
-    
+
     using is_insert_spec_aux_imp_sorted is_insert_spec_aux_imp_mset_eq' 
       is_insert_spec_aux_imp_rest_eq is_insert_spec_aux_imp_length_eq
       insert_spec_aux_preserves_stoppers
@@ -1085,10 +1138,12 @@ context weak_ordering begin
     by auto fastforce
     
     
-  abbreviation "insort_step_cost \<equiv> cost ''icmp_slt'' 1 + cost ''add'' 1 + cost ''is_insert'' 1 + cost ''call'' 1
-     + cost ''if'' 1"  
+abbreviation "insort_step_cost \<equiv> cost ''icmp_slt'' 1 + cost ''add'' 1
+     + cost ''is_insert'' 1 + cost ''call'' 1  + cost ''if'' 1"  
     
-  definition "gen_insertion_sort_unguarded N i\<^sub>0 h xs \<equiv> doN {
+subsection \<open>insertion_sort_unguarded\<close>
+
+  definition "insertion_sort_unguarded N i\<^sub>0 h xs \<equiv> doN {
     ASSERT ((\<forall>i\<in>{i\<^sub>0..<h}. has_stopper N xs i) \<and> h\<le>length xs);
     (xs,_)\<leftarrow>monadic_WHILEIET (\<lambda>(xs',i). 
           i\<^sub>0\<le>i \<and> i\<le>h \<and> length xs'=length xs 
@@ -1109,12 +1164,14 @@ context weak_ordering begin
   }"  
   
     
-  lemma gen_insertion_sort_unguarded_correct: 
-    "\<lbrakk>sorted_wrt_lt (\<^bold><) (take i\<^sub>0 xs); (\<forall>i\<in>{i\<^sub>0..<h}. has_stopper N xs i) \<and> h\<le>length xs ; i\<^sub>0<h; h\<le>length xs \<rbrakk> 
-      \<Longrightarrow> gen_insertion_sort_unguarded N i\<^sub>0 h xs 
+  lemma insertion_sort_unguarded_correct: 
+    "\<lbrakk>sorted_wrt_lt (\<^bold><) (take i\<^sub>0 xs); (\<forall>i\<in>{i\<^sub>0..<h}. has_stopper N xs i) \<and> h\<le>length xs;
+           i\<^sub>0<h; h\<le>length xs \<rbrakk> 
+      \<Longrightarrow> insertion_sort_unguarded N i\<^sub>0 h xs 
         \<le> \<Down>Id (timerefine (TId(''slice_sort'' := enat (h-i\<^sub>0+1) *m insort_step_cost)) (
           slice_sort_spec (\<^bold><) xs 0 h))"
-    unfolding gen_insertion_sort_unguarded_def sort_one_more_spec_unguarded_def slice_sort_spec_def sort_spec_def sorted_sorted_wrt
+    unfolding insertion_sort_unguarded_def sort_one_more_spec_unguarded_def
+          slice_sort_spec_def sort_spec_def sorted_sorted_wrt
     
     apply (intro refine0)
     subgoal by simp
@@ -1137,7 +1194,8 @@ context weak_ordering begin
           apply(simp add: norm_cost)
           apply sc_solve by auto 
       subgoal 
-        apply (clarsimp simp: cost_is_insert_guarded_step_def costmult_add_distrib costmult_cost lift_acost_propagate lift_acost_cost)
+        apply (clarsimp simp: cost_is_insert_guarded_step_def costmult_add_distrib costmult_cost 
+              lift_acost_propagate lift_acost_cost)
         apply sc_solve
         apply (simp add: one_enat_def algebra_simps)
         done
@@ -1156,7 +1214,8 @@ context weak_ordering begin
       apply (rule conjI)
       subgoal
         apply (simp add: lift_acost_diff_to_the_right)
-        apply (clarsimp simp: cost_is_insert_guarded_step_def costmult_add_distrib costmult_cost lift_acost_propagate lift_acost_cost timerefineA_update_apply_same_cost')
+        apply (clarsimp simp: cost_is_insert_guarded_step_def costmult_add_distrib costmult_cost
+                lift_acost_propagate lift_acost_cost timerefineA_update_apply_same_cost')
         apply sc_solve
         apply (auto simp flip: plus_enat_simps simp: algebra_simps one_enat_def plus_enat_simps)
         done
@@ -1165,11 +1224,13 @@ context weak_ordering begin
       done
     done
         
-  definition "gen_insertion_sort_unguarded2 N i h xs \<equiv> doN {
+subsection \<open>insertion_sort_unguarded2\<close>
+
+  definition "insertion_sort_unguarded2 N i h xs \<equiv> doN {
     (xs,_)\<leftarrow>monadic_WHILEIT (\<lambda>_. True)
       (\<lambda>(xs,i). SPECc2 ''icmp_slt'' (<) i h) 
       (\<lambda>(xs,i). doN {
-        xs \<leftarrow> is_insert2_unguarded N xs i;
+        xs \<leftarrow> is_insert_unguarded2 N xs i;
         ASSERT (i<h);
         i \<leftarrow> SPECc2 ''add'' (+) i 1;
         RETURN (xs,i)
@@ -1178,7 +1239,8 @@ context weak_ordering begin
   }"  
   
   definition "TR_is_insert3 N \<equiv> (
-                   (pp (pp (TId(''list_get'' := lift_acost mop_array_nth_cost, ''list_set'' := lift_acost mop_array_upd_cost, ''mop_cmp_v_idx'' := cost ''cmpo_v_idx'' 1))
+                   (pp (pp (TId(''list_get'' := lift_acost mop_array_nth_cost, 
+        ''list_set'' := lift_acost mop_array_upd_cost, ''mop_cmp_v_idx'' := cost ''cmpo_v_idx'' 1))
                          (TId(''is_insert'' := cost_insert N, ''is_insert_g'' := cost_insert_guarded N)))
                      TId))"
 
@@ -1186,7 +1248,7 @@ context weak_ordering begin
   \<^cancel>\<open>
   lemma is_insert3_sorts_one_more_right: 
     assumes "(xs,xs')\<in>slicep_rel l h" "(i,i')\<in>idx_shift_rel l" "i<h" "i'<j'"
-    shows "is_insert2_unguarded N xs i \<le>\<Down>(slice_rel xs l h) (timerefine (TR_is_insert3 N) (sort_one_more_spec_unguarded N xs' i' j'))"
+    shows "is_insert_unguarded2 N xs i \<le>\<Down>(slice_rel xs l h) (timerefine (TR_is_insert3 N) (sort_one_more_spec_unguarded N xs' i' j'))"
   proof -
     note is_insert3_unguarded_correct'
     also note is_insert_unguarded_sorts_one_more
@@ -1199,23 +1261,16 @@ context weak_ordering begin
       done
   qed \<close>
  
-lemma timerefine_mono3: 
-  fixes R :: "_ \<Rightarrow> ('a, enat) acost"
-  assumes "wfR'' R"
-  shows "c\<le>c' \<Longrightarrow> R=R' \<Longrightarrow> timerefine R c \<le> timerefine R' c'"
-  apply simp
-  apply(rule timerefine_mono2)
-  using assms by auto
 
-thm is_insert3_unguarded_correct'
-thm is_insert_unguarded_sorts_one_more
+subsubsection \<open>Refinement Lemma\<close>
 
   lemma is_insert3_sorts_one_more: 
     assumes "(xs,xs')\<in>slicep_rel l h" "(i,i')\<in>idx_shift_rel l" "i<h" "i'<j'"
-    shows "is_insert2_unguarded N xs i \<le>\<Down>(slice_rel xs l h) (timerefine (TR_is_insert3 N) (sort_one_more_spec_unguarded N xs' i' j'))"
+    shows "is_insert_unguarded2 N xs i
+     \<le>\<Down>(slice_rel xs l h) (timerefine (TR_is_insert3 N) (sort_one_more_spec_unguarded N xs' i' j'))"
     using assms apply -
       apply(rule order_trans)
-     apply(rule is_insert3_unguarded_correct'[OF assms(1-3)])
+     apply(rule is_insert_unguarded2_correct'[OF assms(1-3)])
     apply(rule nrest_Rel_mono)
     unfolding TR_is_insert3_def
       apply(subst (2) timerefine_iter2[symmetric])
@@ -1241,12 +1296,15 @@ lemma sp_TR_is_insert3[simp]:"struct_preserving (TR_is_insert3 N)"
   apply(simp add: norm_pp )  by(auto intro!: struct_preserving_upd_I)
   
 
-  lemma gen_insertion_sort_unguarded2_refine: 
+  lemma insertion_sort_unguarded2_refine: 
     "\<lbrakk> (xsi,xs) \<in> slicep_rel l h; (ii,i)\<in>idx_shift_rel l; (ji,j)\<in>idx_shift_rel l \<rbrakk> 
-      \<Longrightarrow> gen_insertion_sort_unguarded2 N ii ji xsi \<le>\<Down>(slice_rel xsi l h) (timerefine (TR_is_insert3 N) (gen_insertion_sort_unguarded N i j xs))"
-    unfolding gen_insertion_sort_unguarded2_def gen_insertion_sort_unguarded_def monadic_WHILEIET_def
-    apply (refine_rcg is_insert3_sorts_one_more monadic_WHILEIT_refine' bindT_refine_conc_time_my_inres SPECc2_refine')
-    supply [refine_dref_RELATES] = RELATESI[of "slice_rel xsi l h \<times>\<^sub>r idx_shift_rel l"] RELATESI[of "idx_shift_rel l"] 
+      \<Longrightarrow> insertion_sort_unguarded2 N ii ji xsi 
+        \<le>\<Down>(slice_rel xsi l h) (timerefine (TR_is_insert3 N) (insertion_sort_unguarded N i j xs))"
+    unfolding insertion_sort_unguarded2_def insertion_sort_unguarded_def monadic_WHILEIET_def
+    apply (refine_rcg is_insert3_sorts_one_more monadic_WHILEIT_refine'
+                    bindT_refine_conc_time_my_inres SPECc2_refine')
+    supply [refine_dref_RELATES] = RELATESI[of "slice_rel xsi l h \<times>\<^sub>r idx_shift_rel l"] 
+                                    RELATESI[of "idx_shift_rel l"] 
     apply refine_dref_type
     apply (clarsimp_all simp: inres_SPECc2)
     
@@ -1269,10 +1327,12 @@ lemma sp_TR_is_insert3[simp]:"struct_preserving (TR_is_insert3 N)"
     
 end
     
+subsection \<open>insertion_sort_unguarded3\<close>
+
 context sort_impl_context begin
 
 
-  definition "gen_insertion_sort_unguarded3 N i h xs \<equiv> doN {
+  definition "insertion_sort_unguarded3 N i h xs \<equiv> doN {
     (xs,_)\<leftarrow>monadic_WHILEIT (\<lambda>_. True)
       (\<lambda>(xs,i). SPECc2 ''icmp_slt'' (<) i h) 
       (\<lambda>(xs,i). doN {
@@ -1284,12 +1344,14 @@ context sort_impl_context begin
     RETURN xs
   }"  
 
+subsubsection \<open>Refinement Lemma\<close>
 
-  lemma gen_insertion_sort_unguarded3_refines:
+  lemma insertion_sort_unguarded3_refines:
     "(i,i')\<in>Id \<Longrightarrow> (h,h')\<in>Id \<Longrightarrow> (xs,xs')\<in>Id
-      \<Longrightarrow> gen_insertion_sort_unguarded3 N i h xs \<le> \<Down>Id (timerefine TR_cmp_swap (gen_insertion_sort_unguarded2 N i' h' xs'))"
+      \<Longrightarrow> insertion_sort_unguarded3 N i h xs 
+            \<le> \<Down>Id (timerefine TR_cmp_swap (insertion_sort_unguarded2 N i' h' xs'))"
     supply conc_Id[simp del]
-    unfolding gen_insertion_sort_unguarded3_def gen_insertion_sort_unguarded2_def
+    unfolding insertion_sort_unguarded3_def insertion_sort_unguarded2_def
     supply [refine] = is_insert_unguarded4_refines
     apply(refine_rcg MIf_refine SPECc2_refine' bindT_refine_conc_time_my_inres monadic_WHILEIT_refine' )
                         apply refine_dref_type
@@ -1299,25 +1361,25 @@ context sort_impl_context begin
   done
 
 
+subsubsection \<open>Synthesize unguarded_insertion_sort_impl\<close>
 
   context fixes N :: nat begin
   sepref_register 
-    unguarded_insertion_sort2: "gen_insertion_sort_unguarded3 N"
+    unguarded_insertion_sort2: "insertion_sort_unguarded3 N"
   end
     
-  sepref_def unguarded_insertion_sort_impl is "uncurry2 (PR_CONST (gen_insertion_sort_unguarded3 N))" 
+  sepref_def unguarded_insertion_sort_impl is "uncurry2 (PR_CONST (insertion_sort_unguarded3 N))" 
     :: "size_assn\<^sup>k *\<^sub>a size_assn\<^sup>k *\<^sub>a (array_assn elem_assn)\<^sup>d \<rightarrow>\<^sub>a array_assn elem_assn"
-    unfolding gen_insertion_sort_unguarded3_def PR_CONST_def
+    unfolding insertion_sort_unguarded3_def PR_CONST_def
     apply (annot_snat_const "TYPE('size_t)")
     by sepref 
     
 end    
     
     
+        
     
-    
-    
-    
+subsection \<open>Insertion sort - specification guarded\<close>
     
     
     
@@ -1356,8 +1418,9 @@ context weak_ordering begin
   abbreviation "insort_guarded_step_cost \<equiv> cost ''icmp_slt'' 1 + cost ''add'' 1 + cost ''is_insert_g'' 1 + cost ''call'' 1
      + cost ''if'' 1"  
   
+subsection \<open>insertion_sort_guarded\<close>
     
-  definition "gen_insertion_sort_guarded i\<^sub>0 h xs \<equiv> doN {
+  definition "insertion_sort_guarded i\<^sub>0 h xs \<equiv> doN {
     ASSERT (h\<le>length xs);
     (xs,_)\<leftarrow>monadic_WHILEIET (\<lambda>(xs',i). 
           i\<^sub>0\<le>i \<and> i\<le>h \<and> length xs'=length xs 
@@ -1377,12 +1440,12 @@ context weak_ordering begin
   }"  
   
     
-  lemma gen_insertion_sort_guarded_correct: 
+  lemma insertion_sort_guarded_correct: 
     "\<lbrakk>sorted_wrt_lt (\<^bold><) (take i\<^sub>0 xs); h\<le>length xs ; i\<^sub>0<h; h\<le>length xs \<rbrakk> 
-      \<Longrightarrow> gen_insertion_sort_guarded i\<^sub>0 h xs 
+      \<Longrightarrow> insertion_sort_guarded i\<^sub>0 h xs 
         \<le> \<Down>Id (timerefine (TId(''slice_sort'' := enat (h-i\<^sub>0+1) *m insort_guarded_step_cost)) (
           slice_sort_spec (\<^bold><) xs 0 h))"
-    unfolding gen_insertion_sort_guarded_def sort_one_more_spec_guarded_def slice_sort_spec_def sort_spec_def sorted_sorted_wrt
+    unfolding insertion_sort_guarded_def sort_one_more_spec_guarded_def slice_sort_spec_def sort_spec_def sorted_sorted_wrt
     
     apply (intro refine0)
     subgoal by simp
@@ -1433,9 +1496,10 @@ context weak_ordering begin
     done
         
     
+subsection \<open>insertion_sort_guarded2\<close>
     
     
-  definition "gen_insertion_sort_guarded2 l i h xs \<equiv> doN {
+  definition "insertion_sort_guarded2 l i h xs \<equiv> doN {
     ASSERT (l \<le> i);
     (xs,_)\<leftarrow>monadic_WHILEIT (\<lambda>_. True)
       (\<lambda>(xs,i). SPECc2 ''icmp_slt'' (<) i h) 
@@ -1451,14 +1515,6 @@ context weak_ordering begin
  
 
  
-  
-  (* TODO: Move, better name *)                     
-  lemma timerefine_R_cf_mono:
-    fixes R :: "_ \<Rightarrow> (_, enat) acost"
-    assumes "wfR'' R'"
-    shows "R\<le>R' \<Longrightarrow> \<Down> S (timerefine R c) \<le> \<Down> S (timerefine R' c)"
-    by (simp add: assms nrest_Rel_mono timerefine_R_mono_wfR'')
-
   (* TODO: enable this kind of reasoning! by fixing timerefine_comm_concfun *)
   \<^cancel>\<open>
   lemma is_insert3_guarded_sorts_one_more_right: 
@@ -1490,51 +1546,24 @@ context weak_ordering begin
       done
   qed\<close>
 
-  thm timerefine_mono2 timerefine_R_mono_wfR''
 
-lemma timerefine_mono_both: 
-  fixes R :: "_ \<Rightarrow> ('c, 'd::{complete_lattice,nonneg,mult_zero,ordered_semiring}) acost"
-  assumes "wfR'' R'"
-    and "R\<le>R'"
-  shows "c\<le>c' \<Longrightarrow> timerefine R c \<le> timerefine R' c'"
-  apply(cases c) apply simp
-  apply(cases c') apply (auto simp: less_eq_acost_def timerefine_def split: nrest.splits option.splits simp: le_fun_def)
-  subgoal  by (metis le_some_optE) 
-  proof (goal_cases)
-    case (1 x2 x2a x x2b x2c xa)
-    then have l: "\<And>ac. the_acost x2b ac \<le>  the_acost x2c ac"
-      apply(cases x2b; cases x2c) unfolding less_eq_acost_def  
-      apply auto
-      by (metis acost.sel less_eq_acost_def less_eq_option_Some)
-    show ?case
-      apply(rule Sum_any_mono)
-      subgoal using l apply(rule ordered_semiring_class.mult_mono)
-        subgoal using assms(2) unfolding le_fun_def
-          by (simp add: the_acost_mono)
-        subgoal by (simp add: needname_nonneg)
-        subgoal
-          by (simp add: needname_nonneg)
-        done
-      apply(rule wfR_finite_mult_left2) by fact
-  qed 
-
-
-lemma fun_upd_parallel_I: "f\<le>f' \<Longrightarrow> y\<le>y' \<Longrightarrow> f(x:=y) \<le> f'(x:=y')"
-  unfolding fun_upd_def le_fun_def  
-  by auto
 
 lemma cost_insert_guarded_mono: "a \<le> b \<Longrightarrow> cost_insert_guarded a \<le> cost_insert_guarded b"
   unfolding cost_insert_guarded_def 
-          unfolding cost_insert_guarded_def cost_is_insert_guarded_step_def
-          apply(auto simp add: norm_pp norm_cost intro!: wfR''_upd )
-          apply sc_solve by auto
+  unfolding cost_insert_guarded_def cost_is_insert_guarded_step_def
+  apply(auto simp add: norm_pp norm_cost intro!: wfR''_upd )
+  apply sc_solve 
+  by auto
 
 lemma cost_insert_mono: "a \<le> b \<Longrightarrow> cost_insert a \<le> cost_insert b"
   unfolding cost_insert_def 
-          unfolding cost_is_insert_step_def
-        apply(auto simp add: norm_pp norm_cost intro!: wfR''_upd )
-          apply sc_solve by auto
+  unfolding cost_is_insert_step_def
+  apply(auto simp add: norm_pp norm_cost intro!: wfR''_upd )
+  apply sc_solve
+  by auto
 
+
+subsubsection \<open>Refinement Lemma\<close>
 
   lemma is_insert3_guarded_sorts_one_more: 
     assumes "(xs,xs')\<in>slicep_rel l h" "(i,i')\<in>idx_shift_rel l" "i<h" "N\<ge>i-l"
@@ -1568,10 +1597,10 @@ lemma cost_insert_mono: "a \<le> b \<Longrightarrow> cost_insert a \<le> cost_in
 
 
 
-  lemma gen_insertion_sort_guarded2_refine: 
+  lemma insertion_sort_guarded2_refine: 
     "\<lbrakk> (xsi,xs) \<in> slicep_rel l h; (ii,i)\<in>idx_shift_rel l; (ji,j)\<in>idx_shift_rel l; j\<le>N \<rbrakk> 
-      \<Longrightarrow> gen_insertion_sort_guarded2 l ii ji xsi \<le>\<Down>(slice_rel xsi l h) (timerefine (TR_is_insert3 N) (gen_insertion_sort_guarded i j xs))"
-    unfolding gen_insertion_sort_guarded2_def gen_insertion_sort_guarded_def monadic_WHILEIET_def
+      \<Longrightarrow> insertion_sort_guarded2 l ii ji xsi \<le>\<Down>(slice_rel xsi l h) (timerefine (TR_is_insert3 N) (insertion_sort_guarded i j xs))"
+    unfolding insertion_sort_guarded2_def insertion_sort_guarded_def monadic_WHILEIET_def
     apply (refine_rcg is_insert3_guarded_sorts_one_more monadic_WHILEIT_refine' bindT_refine_conc_time_my_inres SPECc2_refine')
     supply [refine_dref_RELATES] = 
       RELATESI[of "slice_rel xsi l h \<times>\<^sub>r idx_shift_rel l"] RELATESI[of "idx_shift_rel l"]
@@ -1598,12 +1627,11 @@ lemma cost_insert_mono: "a \<le> b \<Longrightarrow> cost_insert a \<le> cost_in
 end    
     
     
+subsection \<open>insertion_sort_guarded3\<close>
      
 context sort_impl_context begin
-
-  
-    
-  definition "gen_insertion_sort_guarded3 l i h xs \<equiv> doN {
+   
+  definition "insertion_sort_guarded3 l i h xs \<equiv> doN {
     ASSERT (l \<le> i);
     (xs,_)\<leftarrow>monadic_WHILEIT (\<lambda>_. True)
       (\<lambda>(xs,i). SPECc2 ''icmp_slt'' (<) i h) 
@@ -1616,12 +1644,13 @@ context sort_impl_context begin
     RETURN xs
   }"  
 
+subsubsection \<open>Refinement Lemma\<close>
 
-  lemma gen_insertion_sort_guarded3_refines:
+  lemma insertion_sort_guarded3_refines:
     "(l,l')\<in>Id \<Longrightarrow> (i,i')\<in>Id \<Longrightarrow> (h,h')\<in>Id \<Longrightarrow> (xs,xs')\<in>Id
-      \<Longrightarrow> gen_insertion_sort_guarded3 l i h xs \<le> \<Down>Id (timerefine TR_cmp_swap (gen_insertion_sort_guarded2 l' i' h' xs'))"
+      \<Longrightarrow> insertion_sort_guarded3 l i h xs \<le> \<Down>Id (timerefine TR_cmp_swap (insertion_sort_guarded2 l' i' h' xs'))"
     supply conc_Id[simp del]
-    unfolding gen_insertion_sort_guarded3_def gen_insertion_sort_guarded2_def
+    unfolding insertion_sort_guarded3_def insertion_sort_guarded2_def
     supply [refine] = is_insert_guarded4_refines
     apply(refine_rcg MIf_refine SPECc2_refine' bindT_refine_conc_time_my_inres monadic_WHILEIT_refine' )
                         apply refine_dref_type
@@ -1629,332 +1658,19 @@ context sort_impl_context begin
   apply (simp_all (no_asm))
   apply (auto simp: timerefineA_cost)  
   done
-
-
-
   
+subsubsection \<open>synthesize guarded_insertion_sort_impl\<close>
 
+sepref_register
+    guarded_insertion_sort3: "insertion_sort_guarded3"
 
-
-
-  sepref_register    
-    guarded_insertion_sort3: "gen_insertion_sort_guarded3"
-
-  sepref_def guarded_insertion_sort_impl is "uncurry3 (PR_CONST (gen_insertion_sort_guarded3))" 
+  sepref_def guarded_insertion_sort_impl is "uncurry3 (PR_CONST (insertion_sort_guarded3))" 
     :: "size_assn\<^sup>k *\<^sub>a size_assn\<^sup>k *\<^sub>a size_assn\<^sup>k *\<^sub>a (array_assn elem_assn)\<^sup>d \<rightarrow>\<^sub>a array_assn elem_assn"
-    unfolding gen_insertion_sort_guarded3_def PR_CONST_def
+    unfolding insertion_sort_guarded3_def PR_CONST_def
     apply (annot_snat_const "TYPE('size_t)")
     by sepref    
 
 end 
-    
-    
-    
-    
-    
-    
-(*    
-    
-  definition "sort_one_more_spec GUARDED xs i \<equiv> doN {
-      ASSERT (i<length xs \<and> sorted_wrt_lt (\<^bold><) (take i xs));
-      ASSERT (\<not>GUARDED \<longrightarrow> 0<i \<and> \<not>xs!i\<^bold><xs!0); 
-      SPEC (\<lambda>xs'. mset (take (i+1) xs') = mset (take (i+1) xs) \<and> drop (i+1) xs' = drop (i+1) xs \<and> length xs'=length xs \<and> sorted_wrt_lt (\<^bold><) (take (i+1) xs') \<and> (\<not>GUARDED \<longrightarrow> xs'!0 = xs!0))
-    }"  
-    
-  (* For presentation in paper *)  
-  lemma "sort_one_more_spec G xs i = doN {
-      ASSERT (i<length xs \<and> sorted_wrt_lt (\<^bold><) (slice 0 i xs));
-      ASSERT (G \<or> 0<i \<and> \<not>(xs!i\<^bold><xs!0));
-      SPEC (\<lambda>xs'. inres (slice_sort_spec (\<^bold><) xs 0 (i+1)) xs' \<and> (\<not>G \<longrightarrow> xs'!0 = xs!0))
-    }"
-    unfolding slice_sort_spec_def sort_one_more_spec_def
-    apply (simp only: pw_eq_iff refine_pw_simps; safe)
-    apply (simp_all add: Misc.slice_def sort_spec_def)
-    done
-    
-  lemma "sort_one_more_spec G xs i = doN {
-      ASSERT (i<length xs \<and> sorted_wrt_lt (\<^bold><) (slice 0 i xs));
-      ASSERT (G \<or> 0<i \<and> \<not>(xs!i\<^bold><xs!0));
-      SPEC (\<lambda>xs'. sort_spec (\<^bold><) (slice 0 (i+1) xs) (slice 0 (i+1) xs') 
-          \<and> length xs'=length xs 
-          \<and> slice (i+1) (length xs) xs' = slice (i+1) (length xs) xs 
-          \<and> (\<not>G \<longrightarrow> xs'!0 = xs!0))
-    }"
-    unfolding slice_sort_spec_def sort_one_more_spec_def
-    apply (simp only: pw_eq_iff refine_pw_simps; safe)
-    apply (simp_all add: Misc.slice_def sort_spec_def)
-    done
-    
-    
-    
-  lemma conv_idxs_to_drop_eq: "length xs = length ys \<Longrightarrow> (\<forall>j\<in>{n..<length ys}. xs ! j = ys ! j) \<longleftrightarrow> drop n xs = drop n ys"
-    apply (simp add: list_eq_iff_nth_eq)
-    apply (safe;clarsimp)
-    by (metis add_diff_cancel_left' diff_less_mono le_iff_add)
-
-    (*
-  lemma is_insert_sorts_one_more[param_fo, THEN nres_relD,refine]: 
-    "(is_insert_spec GUARDED, sort_one_more_spec GUARDED) 
-        \<in> \<langle>Id\<rangle>list_rel \<rightarrow> nat_rel \<rightarrow> \<langle>\<langle>Id\<rangle>list_rel\<rangle>nres_rel"
-    apply (intro fun_relI nres_relI; auto)    
-    unfolding sort_one_more_spec_def is_insert_spec_alt is_insert_spec_aux_def
-    apply (clarsimp simp: pw_le_iff refine_pw_simps)
-    apply (intro conjI)
-    subgoal sledgehammer sorry
-    subgoal apply (simp add: list_eq_iff_nth_eq)
-    *)
-    
-        
-  lemma is_insert_sorts_one_more[param_fo, THEN nres_relD,refine]: 
-    "(is_insert_spec GUARDED, sort_one_more_spec GUARDED) 
-        \<in> \<langle>Id\<rangle>list_rel \<rightarrow> nat_rel \<rightarrow> \<langle>\<langle>Id\<rangle>list_rel\<rangle>nres_rel"
-    apply (intro fun_relI nres_relI)    
-    using is_insert_spec_aux_imp_sorted is_insert_spec_aux_imp_mset_eq' 
-      is_insert_spec_aux_imp_rest_eq is_insert_spec_aux_imp_length_eq
-    unfolding sort_one_more_spec_def is_insert_spec_alt
-    apply (simp add: pw_le_iff refine_pw_simps)
-    apply (auto simp: )
-    done
-
-      
-  definition "gen_insertion_sort GUARDED i\<^sub>0 h xs \<equiv> doN {
-    ASSERT ((\<not>GUARDED \<longrightarrow> 0<i\<^sub>0) \<and> h\<le>length xs);
-    (xs,_)\<leftarrow>WHILEIT (\<lambda>(xs',i). 
-        i\<^sub>0\<le>i \<and> i\<le>h \<and> length xs'=length xs \<and> mset (take i xs') = mset (take i xs) \<and> drop i xs' = drop i xs \<and> sorted_wrt_lt (\<^bold><) (take i xs')
-      \<and> (\<not>GUARDED \<longrightarrow> xs'!0 = xs!0)
-      ) 
-      (\<lambda>(xs,i). i<h) 
-      (\<lambda>(xs,i). doN {
-        xs \<leftarrow> sort_one_more_spec GUARDED xs i;
-        ASSERT (i<h);
-        let i=i+1;
-        RETURN (xs,i)
-      }) (xs,i\<^sub>0);
-    RETURN xs
-  }"  
-  
-    
-  lemma gen_insertion_sort_correct: 
-    "\<lbrakk>sorted_wrt_lt (\<^bold><) (take i\<^sub>0 xs); \<not>GUARDED \<longrightarrow> 0<i\<^sub>0; i\<^sub>0<h; h\<le>length xs; \<not>GUARDED \<longrightarrow> (\<forall>i\<in>{i\<^sub>0..<h}. \<exists>j<i. i-j<N \<and> \<not>xs!i \<^bold>< xs!j) \<rbrakk> 
-      \<Longrightarrow> gen_insertion_sort GUARDED i\<^sub>0 h xs \<le> slice_sort_spec (\<^bold><) xs 0 h"
-    unfolding gen_insertion_sort_def sort_one_more_spec_def slice_sort_spec_def sort_spec_def sorted_sorted_wrt
-    apply (refine_vcg 
-      WHILEIT_rule[where R="measure (\<lambda>(_,i). length xs - i)"])       
-      
-    apply (all \<open>(clarsimp;fail)?\<close>) 
-    subgoal by clarsimp (metis atLeastLessThan_iff hd_drop_conv_nth less_le_trans)
-    subgoal by clarsimp (metis hd_drop_conv_nth less_le_trans take_Suc_conv_app_nth union_code)
-    subgoal apply clarsimp by (metis drop_Suc tl_drop)
-    subgoal apply simp by force
-    subgoal apply simp by (metis Misc.slice_def drop0 drop_take)
-    subgoal by (clarsimp simp: Misc.slice_def)    
-    done
-
-(*
-  
-  lemma "\<lbrakk>part_sorted_wrt (le_by_lt (\<^bold><)) n xs; sort_spec (\<^bold><) (slice 0 n xs) (slice 0 n xs'); drop n xs' = drop n xs\<rbrakk> 
-    \<Longrightarrow> part_sorted_wrt (le_by_lt (\<^bold><)) n xs'"
-    unfolding sort_spec_def
-    apply auto
-  proof -
-    define xs\<^sub>1 where "xs\<^sub>1 = slice 0 n xs"
-    define xs\<^sub>2 where "xs\<^sub>2 = drop n xs"
-    have "xs = xs\<^sub>1@xs\<^sub>2" unfolding xs\<^sub>1_def xs\<^sub>2_def Misc.slice_def by auto
-    thm part_sorted_concatI
-  
-    
-    
-    unfolding sort_spec_def
-    apply auto
-    
-    
-  oops end end
-*)  
-
-
-      
-  definition "gen_insertion_sort2 GUARDED l i h xs \<equiv> doN {
-    (xs,_)\<leftarrow>WHILET
-      (\<lambda>(xs,i). i<h) 
-      (\<lambda>(xs,i). doN {
-        xs \<leftarrow> is_insert3 GUARDED xs l i;
-        ASSERT (i<h);
-        let i=i+1;
-        RETURN (xs,i)
-      }) (xs,i);
-    RETURN xs
-  }"  
-    
-  lemma is_insert3_sorts_one_more: 
-    assumes "(xs,xs')\<in>slicep_rel l h" "(i,i')\<in>idx_shift_rel l" "i<h"
-    shows "is_insert3 GUARDED xs l i \<le>\<Down>(slice_rel xs l h) (sort_one_more_spec GUARDED xs' i')"
-  proof -
-    note is_insert3_correct' 
-    also note is_insert_sorts_one_more
-    finally show ?thesis using assms by simp
-  qed
-
-  
-  lemma gen_insertion_sort2_refine: 
-    "\<lbrakk> (xsi,xs) \<in> slicep_rel l h; (ii,i)\<in>idx_shift_rel l; (ji,j)\<in>idx_shift_rel l \<rbrakk> 
-      \<Longrightarrow> gen_insertion_sort2 GUARDED l ii ji xsi \<le>\<Down>(slice_rel xsi l h) (gen_insertion_sort GUARDED i j xs)"
-    unfolding gen_insertion_sort_def gen_insertion_sort2_def
-    apply (refine_rcg is_insert3_sorts_one_more)
-    supply [refine_dref_RELATES] = RELATESI[of "slice_rel xsi l h \<times>\<^sub>r idx_shift_rel l"] 
-    apply refine_dref_type
-    apply clarsimp_all
-    applyS (auto simp: idx_shift_rel_def slice_rel_alt eq_outside_range_triv slicep_rel_def)[]
-    applyS (auto simp: idx_shift_rel_def slicep_rel_def)[]
-    applyS (auto simp: idx_shift_rel_def slice_rel_alt) []
-    applyS (auto simp: idx_shift_rel_def slicep_rel_def)[]
-    subgoal
-      apply (clarsimp simp: idx_shift_rel_def slice_rel_alt) []
-      by (erule (1) eq_outside_range_gen_trans; auto)
-    done
-  
-        
-end
-    
-context sort_impl_context begin
-  
-  sepref_register 
-    unguarded_insertion_sort2: "gen_insertion_sort2 False"
-    guarded_insertion_sort2: "gen_insertion_sort2 True"
-    
-  sepref_def unguarded_insertion_sort_impl is "uncurry3 (PR_CONST (gen_insertion_sort2 False))" 
-    :: "size_assn\<^sup>k *\<^sub>a size_assn\<^sup>k *\<^sub>a size_assn\<^sup>k *\<^sub>a (woarray_assn elem_assn)\<^sup>d \<rightarrow>\<^sub>a woarray_assn elem_assn"
-    unfolding gen_insertion_sort2_def PR_CONST_def
-    apply (annot_snat_const "TYPE(size_t)")
-    by sepref
-    
-  sepref_def guarded_insertion_sort_impl is "uncurry3 (PR_CONST (gen_insertion_sort2 True))" 
-    :: "size_assn\<^sup>k *\<^sub>a size_assn\<^sup>k *\<^sub>a size_assn\<^sup>k *\<^sub>a (woarray_assn elem_assn)\<^sup>d \<rightarrow>\<^sub>a woarray_assn elem_assn"
-    unfolding gen_insertion_sort2_def PR_CONST_def
-    apply (annot_snat_const "TYPE(size_t)")
-    by sepref
-    
-end    
-
-(*
-context parameterized_weak_ordering begin  
-
-  definition "is_insert_param GUARDED cparam xs l i \<equiv> doN {
-  
-    ASSERT (i<length xs);
-    
-    \<^cancel>\<open>ASSERT (set xs \<subseteq> cdom);\<close>
-    
-    xs \<leftarrow> mop_to_eo_conv xs;
-    
-    (x,xs) \<leftarrow> mop_eo_extract xs i;
-
-    \<^cancel>\<open>
-    ASSERT (x \<in> cdom);
-    ASSERT (\<forall>x. Some x \<in> set xs \<longrightarrow> x\<in>cdom);
-    \<close>
-      
-    (xs,i)\<leftarrow>monadic_WHILEIT (\<lambda>(xs',i'). True) 
-      (\<lambda>(xs,i). if \<not>GUARDED \<or> i>l then doN {ASSERT (i>0); pcmpo_v_idx2 cparam xs x (i-1)} else RETURN False) (\<lambda>(xs,i). doN {
-        ASSERT (i>0);
-        (t,xs) \<leftarrow> mop_eo_extract xs (i-1);
-        xs \<leftarrow> mop_eo_set xs i t;
-        let i = i-1;
-        RETURN (xs,i)
-      }) (xs,i);
-  
-    xs \<leftarrow> mop_eo_set xs i x;  
-    
-    xs \<leftarrow> mop_to_wo_conv xs;
-    
-    RETURN xs
-  }"
-  
-
-  term is_insert4
-      
-  lemma is_insert_param_refine[refine]:
-    assumes "(xs',xs)\<in>cdom_list_rel cparam"
-    assumes "(l',l)\<in>Id"
-    assumes "(i',i)\<in>Id"
-    shows "is_insert_param GUARDED cparam xs' l' i' \<le>\<Down>(cdom_list_rel cparam) (WO.is_insert3 cparam GUARDED xs l i)"
-    supply [refine_dref_RELATES] = RELATESI[of "cdom_list_rel cparam"] RELATESI[of "cdom_olist_rel cparam"]
-    unfolding is_insert_param_def WO.is_insert3_def
-    apply refine_rcg
-    apply (refine_dref_type)
-    using assms
-    by (auto simp: cdom_list_rel_alt cdom_olist_rel_alt in_br_conv)
-      
-  definition "gen_insertion_sort_param GUARDED cparam l i h xs \<equiv> doN {
-    (xs,_)\<leftarrow>WHILET
-      (\<lambda>(xs,i). i<h) 
-      (\<lambda>(xs,i). doN {
-        xs \<leftarrow> is_insert_param GUARDED cparam xs l i;
-        ASSERT (i<h);
-        let i=i+1;
-        RETURN (xs,i)
-      }) (xs,i);
-    RETURN xs
-  }"  
-
-  lemma gen_insertion_sort_param_refinep[refine]:
-    "\<lbrakk>
-      (l',l)\<in>Id; (i',i)\<in>Id; (h',h)\<in>Id; (xs',xs)\<in>cdom_list_rel cparam
-    \<rbrakk> \<Longrightarrow> gen_insertion_sort_param GUARDED cparam l' i' h' xs' 
-    \<le> \<Down>(cdom_list_rel cparam) (WO.gen_insertion_sort2 cparam GUARDED l i h xs)"
-    unfolding gen_insertion_sort_param_def WO.gen_insertion_sort2_def
-    supply [refine_dref_RELATES] = RELATESI[of "cdom_list_rel cparam"]
-    apply refine_rcg
-    apply refine_dref_type
-    apply auto
-    done
-
-  
-
-end
-
-    
-context parameterized_sort_impl_context begin
-    
-  sepref_register 
-    is_guarded_param_insert3: "is_insert_param True"
-    is_unguarded_param_insert3: "is_insert_param False"
-  
-  sepref_def is_guarded_param_insert_impl is "uncurry3 (PR_CONST (is_insert_param True))" 
-    :: "cparam_assn\<^sup>k *\<^sub>a wo_assn\<^sup>d *\<^sub>a size_assn\<^sup>k *\<^sub>a size_assn\<^sup>k \<rightarrow>\<^sub>a wo_assn"
-    unfolding is_insert_param_def PR_CONST_def
-    apply (simp named_ss HOL_ss:)
-    supply [[goals_limit = 1]]
-    apply (annot_snat_const "TYPE(size_t)")
-    by sepref
-
-  sepref_def is_unguarded_param_insert_impl is "uncurry3 (PR_CONST (is_insert_param False))" 
-    :: "cparam_assn\<^sup>k *\<^sub>a wo_assn\<^sup>d *\<^sub>a size_assn\<^sup>k *\<^sub>a size_assn\<^sup>k \<rightarrow>\<^sub>a wo_assn"
-    unfolding is_insert_param_def PR_CONST_def
-    apply (simp named_ss HOL_ss:)
-    supply [[goals_limit = 1]]
-    apply (annot_snat_const "TYPE(size_t)")
-    by sepref
-  
-
-    
-  sepref_register 
-    unguarded_insertion_sort_param: "gen_insertion_sort_param False"
-    guarded_insertion_sort_param: "gen_insertion_sort_param True"
-    
-  sepref_def unguarded_insertion_sort_param_impl is "uncurry4 (PR_CONST (gen_insertion_sort_param False))" 
-    :: "cparam_assn\<^sup>k *\<^sub>a size_assn\<^sup>k *\<^sub>a size_assn\<^sup>k *\<^sub>a size_assn\<^sup>k *\<^sub>a wo_assn\<^sup>d \<rightarrow>\<^sub>a wo_assn"
-    unfolding gen_insertion_sort_param_def PR_CONST_def
-    apply (annot_snat_const "TYPE(size_t)")
-    by sepref
-    
-  sepref_def guarded_insertion_sort_param_impl is "uncurry4 (PR_CONST (gen_insertion_sort_param True))" 
-    :: "cparam_assn\<^sup>k *\<^sub>a size_assn\<^sup>k *\<^sub>a size_assn\<^sup>k *\<^sub>a size_assn\<^sup>k *\<^sub>a wo_assn\<^sup>d \<rightarrow>\<^sub>a wo_assn"
-    unfolding gen_insertion_sort_param_def PR_CONST_def
-    apply (annot_snat_const "TYPE(size_t)")
-    by sepref
-    
-end
-*)
-*)
+ 
 
 end
